changed memory model

theory/JITPer.thy
@@ -15,617 +15,441 @@ imports
   Main
   rBPFCommType rBPFSyntax rBPFSem
   x64Syntax x64Semantics x64Assembler
-  JITState JITPer2Aux
+   x64DecodeProofAux
+  JITPer_add JITPer_mul  JITPer_exit
 
 begin
 
 
-subsection \<open> JIT rule \<close>
-
-text \<open> return 
-  - the number of jited x64 assembly code
-  - the offset pointing to next pc
-  - the jited x64 binary code \<close>
-definition per_jit_add_reg64_1 :: "bpf_ireg \<Rightarrow> bpf_ireg \<Rightarrow> (nat \<times> u64 \<times> x64_bin) option" where
-"per_jit_add_reg64_1 dst src = (
-  let ins = Paddq_rr (bpf_to_x64_reg dst) (bpf_to_x64_reg src) in
-    Some (1, 1, x64_encode ins) 
-)"
-
-definition per_jit_exit :: "(nat \<times> u64 \<times> x64_bin) option" where
-"per_jit_exit = (
-  let ins = Pret in
-    Some (1, 1, x64_encode ins) 
-)"
-
-
-(*definition per_jit_mul_reg64::"bpf_ireg \<Rightarrow> bpf_ireg \<Rightarrow> (nat \<times> u64 \<times> x64_bin) option" where
-"per_jit_mul_reg64 dst src \<equiv> let ins_list = [Pmovq_rr (bpf_to_x64_reg src) R11, Ppushl_r RDX, Pmulq_r R11, Ppopl RDX] in
-   map_option (\<lambda> l. (5, 1, l)) (x64_encodes_func_suffix ins_list)"*)
-
-definition per_jit_mul_reg64::"bpf_ireg \<Rightarrow> bpf_ireg \<Rightarrow> (nat \<times> u64 \<times> x64_bin) option" where
-"per_jit_mul_reg64 dst src \<equiv> 
-  let ins_list = case (bpf_to_x64_reg dst) of 
-      RAX \<Rightarrow> (x64_encode (Pmovq_rr R11 (bpf_to_x64_reg src))@(x64_encode (Ppushl_r RDX)) @ (x64_encode (Pmulq_r R11)) @ (x64_encode (Ppopl RDX))) |
-      
-      RDX \<Rightarrow> (x64_encode (Pmovq_rr R11 (bpf_to_x64_reg src))@(x64_encode (Ppushl_r RAX)) @ (x64_encode (Pmovq_rr RAX RDX)) 
-                  @ (x64_encode (Pmulq_r R11))@ (x64_encode (Pmovq_rr RDX RAX))@ (x64_encode (Ppopl RAX)))|
-      
-      _   \<Rightarrow> (x64_encode(Pmovq_rr R11 (bpf_to_x64_reg src)))@(x64_encode (Ppushl_r RAX)) @ (x64_encode (Pmovq_rr RAX (bpf_to_x64_reg dst)))
-                  @ (x64_encode (Ppushl_r RDX)) @ (x64_encode (Pmulq_r R11)) @ (x64_encode (Ppopl RDX))
-                  @ (x64_encode (Pmovq_rr (bpf_to_x64_reg dst) RAX)) @ (x64_encode (Ppopl RAX))
-  in let len = case (bpf_to_x64_reg dst) of 
-    RAX \<Rightarrow> 4 |
-    RDX \<Rightarrow> 6 |
-    _ \<Rightarrow> 8
-    in Some (len, 1, ins_list)"
-
-                                               
-fun per_jit_ins ::" bpf_instruction \<Rightarrow> (nat \<times> u64 \<times> x64_bin) option" where
-"per_jit_ins bins = (
-  case bins of
-  BPF_ALU64 BPF_ADD dst (SOReg src) \<Rightarrow> (per_jit_add_reg64_1 dst src) |
-  BPF_EXIT \<Rightarrow> per_jit_exit |
-  BPF_ALU64 BPF_MUL dst (SOReg src) \<Rightarrow> (per_jit_mul_reg64 dst src) |
-  _ \<Rightarrow> None
-)"
-
-fun jitper :: "ebpf_asm \<Rightarrow> (nat \<times> u64 \<times> x64_bin) list option" where
-  "jitper [] = Some []" |
-  "jitper (h#xs) = (case per_jit_ins h of 
-                   None \<Rightarrow> None 
-                 | Some (n, off, x) \<Rightarrow> 
-                     (case jitper xs of 
-                        None \<Rightarrow> None 
-                      | Some res \<Rightarrow> Some ((n, off, x) # res)))"
-
-value "Some ((map the (map per_jit_ins [BPF_ALU64 BPF_ADD BR0 (SOReg BR6),BPF_ALU64 BPF_ADD BR0 (SOReg BR1)])))"
-
-value "jitper [BPF_ALU64 BPF_SUB BR0 (SOReg BR6),BPF_EXIT]"
-
-value "jitper [BPF_ALU64 BPF_MUL BR0 (SOReg BR6)]"
-
-                
-value "snd (snd ((the (jitper [BPF_EXIT,BPF_EXIT]))!(0::nat)))"
-
-value "jitper []"
-
-value "jitper [BPF_ALU64 BPF_SUB BR0 (SOReg BR6),BPF_ALU64 BPF_ADD BR0 (SOReg BR6)]"
-
-value "jitper [BPF_ALU64 BPF_ADD BR0 (SOReg BR6),BPF_ALU64 BPF_SUB BR0 (SOReg BR6)]"
-
-value "jitper [BPF_ALU64 BPF_ADD BR0 (SOReg BR6), BPF_ALU64 BPF_ADD BR0 (SOReg BR6), BPF_EXIT]"
-
-value "per_jit_ins (BPF_ALU64 BPF_ADD BR0 (SOReg BR6))"
-
-
-subsection \<open> simulation relation \<close>
-
-definition match_stack :: "regset \<Rightarrow> mem \<Rightarrow> bool" where
-"match_stack xrs m = (
-  \<exists> v. Mem.loadv M64 m ((xrs SP) + (u64_of_memory_chunk M64)) = Some (Vlong v))"
-
-text \<open> because jited x64 code may use pop and push to save registers,
-then x64 memory has more info than sbpf memory \<close>
-(*(Mem.loadv mc bm (Vlong addr) = Some v) \<longrightarrow> (Mem.loadv mc xm (Vlong addr) = Some v))*)
-definition match_mem :: "mem \<Rightarrow> mem \<Rightarrow> bool" where
-"match_mem bm xm = (
-  \<forall> mc addr v. (Mem.loadv mc bm addr = Some v) \<longrightarrow> (Mem.loadv mc xm addr = Some v))"
-
-definition match_reg :: "reg_map \<Rightarrow> regset \<Rightarrow> bool" where
-  "match_reg rm rs = (\<forall> r. (rm r) = rs (bpf_to_x64_reg r))"
-
-definition match_state :: "sbpf_state \<Rightarrow> x64_state \<Rightarrow> bool" where
-"match_state bst xst = (
-  case bst of
-  SBPF_OK pc rs m \<Rightarrow> (
-    case xst of
-      Next xpc xrs xm \<Rightarrow>
-        match_reg rs xrs \<and> \<comment>\<open> for ALU + MEM + Call \<close>
-        match_mem m xm  \<comment>\<open> for MEM + Call \<close> \<and> 
-        match_stack xrs xm |
-      _ \<Rightarrow> False
-  ) |
-  SBPF_Success v \<Rightarrow>(
-    case xst of
-    Next xpc xrs xm \<Rightarrow> v = xrs (bpf_to_x64_reg BR0) \<comment>\<open> for EXIT \<close> |
-      _ \<Rightarrow> False
-  ) |
-  _ \<Rightarrow> False
-)"
-
-lemma sbpf_sem_induct: 
-  "sbpf_sem (m+n) prog s = s' \<Longrightarrow>
-    \<exists> temps.
-    sbpf_sem m prog s = temps \<and> 
-    sbpf_sem n prog temps = s'"
-  apply (induct m arbitrary: n prog s s')
-  apply simp_all
-  done
-
-lemma sbpf_sem_add: 
-  "sbpf_sem (m+n) prog s = s' \<Longrightarrow>
-    s = (SBPF_OK pc rs mem) \<Longrightarrow>
-    s'\<noteq> SBPF_Err \<Longrightarrow>
-    \<exists> temps.
-    sbpf_sem m prog s = temps \<and> 
-    sbpf_sem n prog temps = s'"
-  using sbpf_sem_induct by blast
-
-lemma sbpf_sem_err: 
-  "sbpf_sem (m+n) prog s = s' \<Longrightarrow>
-    s = SBPF_Err \<Longrightarrow>
-    \<exists> temps.
-    sbpf_sem m prog s = temps \<and> 
-    sbpf_sem n prog temps = s'"
-  using sbpf_sem_induct by blast
-
-lemma err_is_still_err:" sbpf_sem x prog SBPF_Err = s' \<Longrightarrow> s' = SBPF_Err "
-  apply(induct x, simp)
-  by auto
-
-lemma suc_success_is_err:"x > 0 \<Longrightarrow> sbpf_sem x prog (SBPF_Success v) = s' \<Longrightarrow> s' = SBPF_Err "
-  apply(induct x, simp)
-  using err_is_still_err by force
-
-lemma intermediate_step_is_ok:"sbpf_sem x prog s = s' \<Longrightarrow> x > 0 \<Longrightarrow> s' \<noteq> SBPF_Err \<Longrightarrow> \<exists> pc rs mem. s = (SBPF_OK pc rs mem)"
-  apply(induct x arbitrary: prog s s')
-  apply simp 
-  using err_is_still_err suc_success_is_err
-  by (metis sbpf_step.elims)
-
-lemma aluq_subgoal_rr_aux1:
-     "bins = BPF_ALU64 BPF_ADD dst (SOReg src) \<Longrightarrow>
-     xins = Paddq_rr (bpf_to_x64_reg dst) (bpf_to_x64_reg src) \<Longrightarrow>
-     prog!(unat pc) = bins \<Longrightarrow>
-     sbpf_step prog (SBPF_OK pc rs m) = (SBPF_OK pc' rs' m')  \<Longrightarrow>
-     Next spc' reg' xm' = exec_instr xins sz spc reg xm \<Longrightarrow>
-     reg (bpf_to_x64_reg dst) = rs dst \<Longrightarrow>
-     reg (bpf_to_x64_reg src) = rs src \<Longrightarrow>
-     reg' (bpf_to_x64_reg dst) = (rs' dst)"
-  apply (unfold exec_instr_def step)
-  apply simp
-  apply(cases "prog ! unat pc",simp_all)
-  subgoal for x91 apply(simp split:if_split_asm) 
-    apply(unfold eval_alu_def eval_reg_def,simp_all)
-    by auto
-  done
-
-
-lemma aluq_subgoal_rr_aux2_1:"xins = Paddq_rr dst src \<Longrightarrow> 
-  Next pc' reg' m' = exec_instr xins sz pc reg m \<Longrightarrow>
-  \<forall> r \<noteq> dst. reg' r = reg r"
-  by (simp add: exec_instr_def)
-
-
-lemma aluq_subgoal_rr_aux2:"xins = Paddq_rr (bpf_to_x64_reg dst) (bpf_to_x64_reg src) \<Longrightarrow> 
-  Next pc' reg' m' = exec_instr xins sz pc reg m \<Longrightarrow>
-  \<forall> r \<noteq> dst. reg' (bpf_to_x64_reg r) = reg (bpf_to_x64_reg r)"
-  using aluq_subgoal_rr_aux2_1 by simp
-
-
-
-lemma aluq_subgoal_rr_aux3:"bins = BPF_ALU64 BPF_ADD dst (SOReg src) \<Longrightarrow> 
-  sbpf_step prog (SBPF_OK pc rs m) = (SBPF_OK pc' rs' m') \<Longrightarrow> 
-  prog!(unat pc) = bins \<Longrightarrow>
-  \<forall> r \<noteq> dst. rs' r = rs r"
-  apply(cases bins,simp_all)
-  apply(cases "prog ! unat pc", simp_all)
-  subgoal for x91 apply(simp split:if_split_asm) 
-    apply(unfold eval_alu_def eval_reg_def,simp_all)
-    by auto
-  done
-
-
-lemma reg_r11_consist:"r = (bpf_to_x64_reg dst) \<Longrightarrow> r \<noteq> x64Syntax.R11"
-  apply(cases dst) 
-  by (unfold bpf_to_x64_reg_corr bpf_to_x64_reg_def, simp_all)
-
-lemma reg_rsp_consist:"r = (bpf_to_x64_reg dst) \<Longrightarrow> r \<noteq> x64Syntax.RSP"
-  apply(cases dst) 
-  by (unfold bpf_to_x64_reg_corr bpf_to_x64_reg_def, simp_all)
-
-lemma mulq_subgoal_rr_aux1_1:
-  "xins = [(3,Pmovq_rr R11 (bpf_to_x64_reg src)), (1,Ppushl_r RAX), (3,Pmovq_rr RAX RDX), (3,Pmulq_r R11), (3,Pmovq_rr RDX RAX), (1,Ppopl RAX)] \<Longrightarrow>
-    exec_instr (snd(xins!0)) (of_nat(fst(xins!0))) pc rs xm = Next pc1 rs1 m1\<and>
-    exec_instr (snd(xins!1)) (of_nat(fst(xins!1))) pc1 rs1 m1 = Next pc2 rs2 m2 \<and>
-    exec_instr (snd(xins!2)) (of_nat(fst(xins!2))) pc2 rs2 m2 = Next pc3 rs3 m3 \<and>
-    exec_instr (snd(xins!3)) (of_nat(fst(xins!3))) pc3 rs3 m3 = Next pc4 rs4 m4 \<and>
-    exec_instr (snd(xins!4)) (of_nat(fst(xins!4))) pc4 rs4 m4 = Next pc5 rs5 m5 \<and> 
-    exec_instr (snd(xins!5)) (of_nat(fst(xins!5))) pc5 rs5 m5 = Next pc6 rs6 m6  \<Longrightarrow>
-   \<forall> r. bpf_to_x64_reg r \<notin> {RDX, RAX} \<longrightarrow> rs (bpf_to_x64_reg r) = rs6 (bpf_to_x64_reg r) "
-  apply(unfold exec_instr_def)
-  apply(cases "Pmulq_r (bpf_to_x64_reg src)",simp_all)
-  subgoal for x6
-    apply(unfold exec_push_def exec_pop_def exec_ret_def  Let_def) 
-    using store_load_consistency
-    apply(cases "storev M64 m1 (rs1 SP - u64_of_memory_chunk M64) (Vlong (rs1 RAX))",simp_all)
-    apply(cases "loadv M64 m5 (rs5 SP)", simp_all)
-    subgoal for a apply(cases a,simp_all)
-      subgoal for x5 
-        apply(cases M64,simp_all)
-        using store_load_consistency reg_r11_consist reg_rsp_consist by auto
-      done
-    done
-  done
-
-lemma mulq_subgoal_rr_aux1_2:
-     "(bpf_to_x64_reg dst) = RDX \<Longrightarrow>
-     bins = BPF_ALU64 BPF_MUL dst (SOReg src) \<Longrightarrow>
-     prog!(unat pc) = bins \<Longrightarrow>
-     sbpf_step prog (SBPF_OK pc reg m) = (SBPF_OK pc' reg' m')  \<Longrightarrow>
-     xins = [(3,Pmovq_rr R11 (bpf_to_x64_reg src)), (1,Ppushl_r RAX), (3,Pmovq_rr RAX RDX), (3,Pmulq_r R11), (3,Pmovq_rr RDX RAX), (1,Ppopl RAX)] \<Longrightarrow>
-    exec_instr (snd(xins!0)) (of_nat(fst(xins!0))) xpc rs xm = Next pc1 rs1 m1\<and>
-    exec_instr (snd(xins!1)) (of_nat(fst(xins!1))) pc1 rs1 m1 = Next pc2 rs2 m2 \<and>
-    exec_instr (snd(xins!2)) (of_nat(fst(xins!2))) pc2 rs2 m2 = Next pc3 rs3 m3 \<and>
-    exec_instr (snd(xins!3)) (of_nat(fst(xins!3))) pc3 rs3 m3 = Next pc4 rs4 m4 \<and>
-    exec_instr (snd(xins!4)) (of_nat(fst(xins!4))) pc4 rs4 m4 = Next pc5 rs5 m5 \<and> 
-    exec_instr (snd(xins!5)) (of_nat(fst(xins!5))) pc5 rs5 m5 = Next pc6 rs6 m6 \<Longrightarrow>
-     rs (bpf_to_x64_reg dst) = reg dst \<Longrightarrow>
-     rs (bpf_to_x64_reg src) = reg src \<Longrightarrow>
-     rs6 (bpf_to_x64_reg dst) = (reg' dst)"
-    apply (unfold exec_instr_def step) 
-    apply(cases "snd (xins ! 0)",simp_all)
-    subgoal for x51
-      apply(unfold exec_push_def exec_pop_def exec_ret_def  Let_def eval_alu_def  eval_reg_def) 
-      apply(split if_splits,simp_all)
-      apply(cases " prog ! unat pc ",simp_all)
-      subgoal for x91 apply(split if_splits,simp_all)
-        using store_load_consistency
-        apply(cases "storev M64 m1 (rs1 SP - u64_of_memory_chunk M64) (Vlong (rs1 RAX))",simp_all)
-        apply(cases "loadv M64 m5 (rs5 SP)", simp_all)
-    subgoal for a apply(cases a,simp_all)
-      subgoal for x5 
-        apply(cases M64,simp_all)
-       by auto
-      done
-    done
-  done
-  done
-
-lemma mulq_subgoal_rr_aux1_3:
-  assumes a0:"xins = [(3,Pmovq_rr R11 (bpf_to_x64_reg src)), (1,Ppushl_r RAX), (3,Pmovq_rr RAX RDX), (3,Pmulq_r R11), (3,Pmovq_rr RDX RAX), (1,Ppopl RAX)]" and
-  a1:"exec_instr (snd(xins!0)) (of_nat(fst(xins!0))) xpc xrs m   = Next xpc1 xrs1 m1" and
-  a2:"exec_instr (snd(xins!1)) (of_nat(fst(xins!1))) xpc1 xrs1 m1 = Next xpc2 xrs2 m2" and
-  a3:"exec_instr (snd(xins!2)) (of_nat(fst(xins!2))) xpc2 xrs2 m2 = Next xpc3 xrs3 m3" and
-  a4:"exec_instr (snd(xins!3)) (of_nat(fst(xins!3))) xpc3 xrs3 m3 = Next xpc4 xrs4 m4" and
-  a5:"exec_instr (snd(xins!4)) (of_nat(fst(xins!4))) xpc4 xrs4 m4 = Next xpc5 xrs5 m5" and
-  a6:"exec_instr (snd(xins!5)) (of_nat(fst(xins!5))) xpc5 xrs5 m5 = Next xpc6 xrs6 m6" 
-  shows "xrs6 RAX = xrs RAX \<and> xrs6 RSP = xrs RSP"
+lemma demo1: 
+  assumes a0:"s' = sbpf_step prog s" and
+  a1:"s = (SBPF_OK pc rs m)" and
+  a2:"s' = (SBPF_OK pc' rs' m')" and
+  a3:"xst = (Next xpc xrs xm)" and
+  a4:"match_state s xst" and
+  a5:"jitper prog = Some x64_prog" and                      
+  a6:"prog \<noteq> [] \<and> unat pc < length prog \<and> unat pc \<ge> 0" and
+  a7:"xpc = 0"
+shows "\<exists> xst'. let l = (x64_prog!(unat pc)) in x64_sem (fst l) (snd (snd l)) xst = xst' \<and> 
+  match_state s' xst'"
+(* \<and> snd xst' = unat (pc+1)*)
 proof-
-  have b1:"m1 = m" using  a0 exec_instr_def a1 by simp
-  have c1:"xrs SP = xrs1 SP" using a0 exec_instr_def a1 by auto
-  have d1:"xrs RAX = xrs1 RAX" using a0 exec_instr_def a1 by auto
+  let "?bpf_ins" = "prog!(unat pc)"
+  have b0:"length prog \<noteq> 0" using a6 by blast
+  have b1:"\<exists> src dst. ?bpf_ins = BPF_ALU64 BPF_ADD dst (SOReg src) \<or> ?bpf_ins = BPF_ALU64 BPF_MUL dst (SOReg src)" using a0 a1 a2 a6 b0 aux1 by blast
+  obtain src dst where b2:"?bpf_ins = BPF_ALU64 BPF_ADD dst (SOReg src) \<or> ?bpf_ins = BPF_ALU64 BPF_MUL dst (SOReg src)" using b1 by blast
+  show ?thesis
+  proof (cases "?bpf_ins = BPF_ALU64 BPF_ADD dst (SOReg src)")
+    case True
+    let "?l_bin"= "snd (snd (the (per_jit_ins ?bpf_ins)))"
+    have c0:"?l_bin = snd (snd (the (per_jit_add_reg64_1 dst src)))" using b2 True by fastforce
+    have c1:"?l_bin = x64_encode (Paddq_rr (bpf_to_x64_reg dst) (bpf_to_x64_reg src))" using per_jit_add_reg64_1_def c0 by fastforce
+    have c2:"snd (snd (x64_prog!(unat pc))) = ?l_bin" using a6 c0 a5 aux5 by metis
+    let "?st" = "x64_sem (fst (x64_prog!(unat pc))) ?l_bin xst"
+    have "x64_prog!(unat pc) = the (per_jit_ins ?bpf_ins)" using aux5 a5 a6 by blast
+    then have "x64_prog!(unat pc) = the (per_jit_add_reg64_1 dst src)" using b2 True by simp
+    then have c3_1:"(fst (x64_prog!(unat pc))) = 1" using per_jit_add_reg64_1_def by simp
+    moreover have "list_in_list ?l_bin 0 ?l_bin" using  list_in_list_prop by simp
+    hence "\<exists> xins2. x64_decode 0 ?l_bin = Some (length ?l_bin, xins2) " 
+      using x64_encode_decode_consistency a3 a7 c1 list_in_list_prop c3_1 by blast
+    then obtain xins2 where c3:"x64_decode 0 ?l_bin = Some (length ?l_bin, xins2)" by auto
+    have c4:"?st = exec_instr xins2 (of_nat (length ?l_bin)) xpc xrs xm" using c3 True a3 a7
+      apply(cases xst,simp_all) apply(cases "prog ! unat pc",simp_all) by (simp add: calculation)
+    have c5:"xins2 = Paddq_rr (bpf_to_x64_reg dst) (bpf_to_x64_reg src)" using Pair_inject c4 c3 c1 option.inject x64_encode_decode_consistency list_in_list_prop by metis
+    have c6:"\<exists> xrs' xpc' xm'. ?st = Next xpc' xrs' xm'" using exec_instr_def spec c5 c4 by auto
+    obtain xrs' xpc' xm' where c7:"?st = Next xpc' xrs' xm'" using c6 by auto
+    have "match_state s' ?st" using addq_subgoal_rr_generic a0 a1 a2 c7 a4 a3 per_jit_add_reg64_1_def b2 c4 c3 True by fastforce
+    then show ?thesis using True b2 c2 by force                                        
+  next
+    case False
+    have c0_1:"?bpf_ins = BPF_ALU64 BPF_MUL dst (SOReg src)" using False b2 by blast
+    let "?l_bin"= "snd (snd (the (per_jit_ins ?bpf_ins)))"
+    have c0:"?l_bin = snd (snd (the (per_jit_mul_reg64 dst src)))" using b2 False by fastforce
+    let "?result" = "per_jit_mul_reg64 dst src"
+    have c2_0:"(bpf_to_x64_reg dst) = RDX \<or> (bpf_to_x64_reg dst) = RAX \<or> (bpf_to_x64_reg dst) \<notin> {RAX, RDX}" by blast
+    
+ thus ?thesis
+ proof(cases "(bpf_to_x64_reg dst) = RDX")
+  case True
+    have c2:"(bpf_to_x64_reg dst) = RDX " using True by blast
+    have c1:"?l_bin = (x64_encode (Pmovq_rr R11 (bpf_to_x64_reg src))@(x64_encode (Ppushl_r RAX)) @ (x64_encode (Pmovq_rr RAX RDX)) 
+                  @ (x64_encode (Pmulq_r R11))@(x64_encode (Pmovq_rr RDX RAX))@(x64_encode (Ppopl RAX)))" 
+      using c0 per_jit_mul_reg64_def c2 by auto
 
-  have b2_1:"Next xpc2 xrs2 m2 = exec_push xpc1 1 M64 m1 xrs1 (xrs1 RAX)" using exec_instr_def exec_push_def a0 a2 by auto
-  let "?addr" = "(xrs1 SP)- (u64_of_memory_chunk M64)"
-  have b2_2:"storev M64 m1 ?addr (Vlong (xrs1 RAX)) \<noteq> None" 
-    using a0 a1 exec_push_def apply(cases "storev M64 m ?addr (Vlong (xrs1 RAX))",simp_all)
-    apply (metis (no_types, lifting) memory_chunk.simps(16) storev_def val.simps(29))    
-    subgoal for a using b1 by blast
+
+    let "?l_bin1" = "x64_encode (Pmovq_rr R11 (bpf_to_x64_reg src))"
+    let "?l_bin2" = "x64_encode (Ppushl_r RAX)"
+    let "?l_bin3" = "x64_encode (Pmovq_rr RAX RDX)"
+    let "?l_bin4" = "x64_encode (Pmulq_r R11)"
+    let "?l_bin5" = "x64_encode (Pmovq_rr RDX RAX)"
+    let "?l_bin6" = "x64_encode (Ppopl RAX)"
+    have d1:"list_in_list (?l_bin1@?l_bin2@?l_bin3@?l_bin4@?l_bin5@?l_bin6) (0::nat) ?l_bin " using c1 list_in_list_prop c1 by metis
+    have d2:"list_in_list ?l_bin 0 ?l_bin = 
+      (list_in_list ?l_bin1 0 ?l_bin \<and> list_in_list ?l_bin2 (0 + length ?l_bin1) ?l_bin \<and> 
+       list_in_list ?l_bin3 (0 + length ?l_bin1+length ?l_bin2) ?l_bin \<and> 
+       list_in_list ?l_bin4 (0 + length ?l_bin1+length ?l_bin2+length ?l_bin3) ?l_bin \<and>
+       list_in_list ?l_bin5 (0 + length ?l_bin1+length ?l_bin2+length ?l_bin3+length ?l_bin4) ?l_bin \<and> 
+       list_in_list ?l_bin6 (0 + length ?l_bin1+length ?l_bin2+length ?l_bin3+length ?l_bin4+length ?l_bin5) ?l_bin)" 
+    using list_in_list_concat d1 c1 list_in_list_prop by (smt (verit, ccfv_SIG))
+
+  have d0:"list_in_list ?l_bin1 0 ?l_bin" using c1 by simp
+  have "\<exists> sz1 xins1. x64_decode 0 ?l_bin = Some (sz1,xins1)" using d0 x64_encode_decode_consistency by blast
+  then obtain sz1 xins1 where d3_0:"x64_decode 0 ?l_bin = Some (sz1,xins1)" by auto
+  hence d0_1:"(sz1,xins1) = (3, Pmovq_rr R11 (bpf_to_x64_reg src))" using d0 x64_encode_decode_consistency by fastforce
+  have "\<exists> xpc1 xrs1 m1. exec_instr xins1 (of_nat sz1) xpc xrs xm = Next xpc1 xrs1 m1" 
+    using d0_1 exec_instr_def by(cases xins1,simp_all)
+  then obtain xpc1 xrs1 m1 where b3:"exec_instr xins1 (of_nat sz1) xpc xrs xm = Next xpc1 xrs1 m1" by blast
+  have f0:"3 = length ?l_bin1" using d0_1 by simp
+
+  have d3:"list_in_list ?l_bin2 (0 + length ?l_bin1) ?l_bin" using d1 d2 c1 by argo
+  have "\<exists> sz2 xins2. x64_decode (0 + length ?l_bin1) ?l_bin = Some (sz2,xins2)" using  d0 c1 x64_encode_decode_consistency 
+    using d3 by blast
+  then obtain sz2 xins2 where d4_0:"x64_decode (0 + length ?l_bin1) ?l_bin = Some (sz2,xins2)" by auto
+  hence d4_1:"(sz2,xins2) =(length ?l_bin2,Ppushl_r RAX)" using x64_encode_decode_consistency c1 d0 option.sel d3 by metis
+  hence d4_2:"sz2 = 1 " apply(cases xins2,simp_all)using bitfield_insert_u8_def Let_def construct_rex_to_u8_def by simp
+  have f1:"1 = length ?l_bin2" using d4_2 d4_1 by blast
+  let "?len" = "length (let rex::8 word = construct_rex_to_u8 False False False False; op::8 word = bitfield_insert_u8 (0::nat) (3::nat) (80::8 word) (0::8 word) in if rex = (64::8 word) then [op] else [rex, op])" 
+  have fn:"?len = 1" by(unfold Let_def construct_rex_to_u8_def bitfield_insert_u8_def,simp_all)
+  have "\<exists> st2. exec_instr xins2 (of_nat sz2) xpc1 xrs1 m1 = st2" 
+    using d4_1 d4_2 apply(unfold exec_instr_def) 
+    by(cases xins2,simp_all)
+  then obtain st2 where d4_3:"exec_instr xins2 (of_nat sz2) xpc1 xrs1 m1 = st2" by auto
+  hence "\<exists> xpc2 xrs2 m2. Next xpc2 xrs2 m2 = st2"
+    apply(unfold exec_instr_def) 
+    apply(cases xins2,simp_all) using d4_1 d4_2 d4_3 fn
+         apply(unfold exec_push_def Let_def,simp_all)
+    apply(cases "storev M64 m1 (Vptr ?len (xrs1 SP - u64_of_memory_chunk M64)) (Vlong (xrs1 RAX))",simp_all)
+    subgoal for x3 
+      apply(unfold storev_def,simp_all)
+      by (meson option.simps(3))
+    subgoal for x3 a 
+      apply(unfold storev_def,simp_all)
+      by blast
     done
-  have b2:"storev M64 m1 ?addr (Vlong (xrs1 RAX)) = Some m2" 
-    using b2_2 b2_1 exec_push_def
-    by(cases "storev M64 m1 ?addr (Vlong (xrs1 RAX))",simp_all)
-  have c2:"xrs2 RSP = ?addr" using b2_1 exec_push_def b2_2 b2_1
-    by(cases "storev M64 m1 ?addr (Vlong (xrs1 RAX))",simp_all) 
-  have d2:"xrs2 RAX = xrs1 RAX" using a0 exec_instr_def a2 b2_1 exec_push_def 
-    by(cases "storev M64 m1 ?addr (Vlong (xrs1 RAX))",simp_all) 
+  then obtain xpc2 xrs2 m2 where b4:"Next xpc2 xrs2 m2 = exec_instr xins2 (of_nat sz2) xpc1 xrs1 m1" using d4_3 by auto
+
+  have d5:"list_in_list ?l_bin3 (0 + length ?l_bin1+length ?l_bin2) ?l_bin" using d1 c1 d2 by metis
+  hence "\<exists> sz3 xins3. x64_decode (0 + length ?l_bin1+length ?l_bin2) ?l_bin = Some (sz3,xins3)" using c1 x64_encode_decode_consistency by blast
+  then obtain sz3 xins3 where d5_1:"x64_decode (0 + length ?l_bin1+length ?l_bin2) ?l_bin = Some (sz3,xins3)" by auto
+  have d6:"(sz3,xins3) = (length ?l_bin3, Pmovq_rr RAX RDX)" using x64_encode_decode_consistency c1 d3 option.sel d0 d5 d5_1 by metis
+  hence d7:"sz3 = 3" by auto
+  have f2:"length ?l_bin3 = 3" using d6 d7 by simp
+  have "\<exists> xpc3 xrs3 m3. exec_instr xins3 (of_nat sz3) xpc2 xrs2 m2 = Next xpc3 xrs3 m3" 
+    using d6 d7 apply(unfold exec_instr_def) 
+    by(cases xins3,simp_all)  
+  then obtain xpc3 xrs3 m3 where b5:"exec_instr xins3 (of_nat sz3) xpc2 xrs2 m2 = Next xpc3 xrs3 m3" by auto
+
+
+  have d8:"list_in_list ?l_bin4 (0 + length ?l_bin1+length ?l_bin2+length ?l_bin3) ?l_bin" using d1 d2 c1 by metis
+  hence "\<exists> sz4 xins4. x64_decode (0 + length ?l_bin1+length ?l_bin2+length ?l_bin3) ?l_bin = Some (sz4,xins4)" 
+    using c1 x64_encode_decode_consistency by blast
+  then obtain sz4 xins4 where d8_1:"x64_decode (0 + length ?l_bin1+length ?l_bin2+length ?l_bin3) ?l_bin = Some (sz4,xins4)" by auto
+  have d9:"(sz4,xins4) = (length ?l_bin4, Pmulq_r R11)" using x64_encode_decode_consistency c1 d3 option.sel d0 d5 d8 d8_1 by metis
+  hence d10:"sz4 = 3" by auto
+  have f3:"length ?l_bin5 = 3" using d10 d8_1 by simp
+  have "\<exists> xpc4 xrs4 m4. exec_instr xins4 (of_nat sz4) xpc3 xrs3 m3 = Next xpc4 xrs4 m4" 
+    using d9 d10 apply(unfold exec_instr_def)
+    by(cases xins4,simp_all)  
+  then obtain xpc4 xrs4 m4 where b6:"exec_instr xins4 (of_nat sz4) xpc3 xrs3 m3 = Next xpc4 xrs4 m4" by auto
+
+
+  have d11:"list_in_list ?l_bin5 (0 + length ?l_bin1+length ?l_bin2+length ?l_bin3+length ?l_bin4) ?l_bin" using d1 d2 c1 by metis
+  hence "\<exists> sz5 xins5. x64_decode (0 + length ?l_bin1+length ?l_bin2+length ?l_bin3+length ?l_bin4) ?l_bin = Some (sz5,xins5)" 
+    using c1 x64_encode_decode_consistency by blast
+  then obtain sz5 xins5 where d11_1:"x64_decode (0 + length ?l_bin1+length ?l_bin2+length ?l_bin3+length ?l_bin4) ?l_bin = Some (sz5,xins5)" by auto
+  have d12:"(sz5,xins5) = (length ?l_bin5, Pmovq_rr RDX RAX)" using x64_encode_decode_consistency c1 d3 option.sel d0 d5 d8 d9 d11 d11_1 by metis
+  hence d13:"sz5 = 3" by auto
+  have f4:"length ?l_bin5 = 3" using d13 d11_1 by simp
+  have "\<exists> xpc5 xrs5 m5. exec_instr xins5 (of_nat sz5) xpc4 xrs4 m4 = Next xpc5 xrs5 m5"
+    using d12 d13 apply(unfold exec_instr_def)
+    by(cases xins5,simp_all)  
+  then obtain xpc5 xrs5 m5 where b7:"exec_instr xins5 (of_nat sz5) xpc4 xrs4 m4 = Next xpc5 xrs5 m5" by auto
+
+ 
+  have d14:"list_in_list ?l_bin6 (0 + length ?l_bin1+length ?l_bin2+length ?l_bin3+length ?l_bin4+length ?l_bin5) ?l_bin" using d1 d2 c1 by metis
+  hence "\<exists> sz6 xins6. x64_decode (0 + length ?l_bin1+length ?l_bin2+length ?l_bin3+length ?l_bin4+length ?l_bin5) ?l_bin = Some (sz6,xins6)" 
+    using c1 x64_encode_decode_consistency by blast
+  then obtain sz6 xins6 where d14_1:"x64_decode (0 + length ?l_bin1+length ?l_bin2+length ?l_bin3+length ?l_bin4+length ?l_bin5) ?l_bin = Some (sz6,xins6)" by auto
+  have d15:"(sz6,xins6) = (length ?l_bin6, Ppopl RAX)" using x64_encode_decode_consistency c1 d3 option.sel d0 d5 d8 d9 d11 d14 d14_1 by metis
+  hence d16:"sz6 = 1" apply(cases xins6,simp_all)using bitfield_insert_u8_def Let_def construct_rex_to_u8_def by simp
+  have f5:"length ?l_bin6 = 1" using d16 d14_1 by (metis d15 prod.inject)
+  have "\<exists> st6. exec_instr xins6 (of_nat sz6) xpc5 xrs5 m5 = st6"
+    using d15 d16 by(cases xins6,simp_all) 
+  then obtain st6 where b8_1:"exec_instr xins6 (of_nat sz6) xpc5 xrs5 m5 = st6" by auto
+  (*hence "\<exists> xpc6 xrs6 m6. st6 = Next xpc6 xrs6 m6"*)
   
-  have b3:"m2=m3" using a0 exec_instr_def a3 by simp
-  have c3:"xrs2 RSP = xrs3 RSP" using  a0 exec_instr_def a3 by auto
+  let "?xins" = "[(sz1,xins1)]@[(sz2,xins2)]@[(sz3,xins3)]@[(sz4,xins4)]@[(sz5,xins5)]@[(sz6,xins6)]"
+  have c13:"?xins = [(3,Pmovq_rr R11 (bpf_to_x64_reg src)), (1,Ppushl_r RAX), (3,Pmovq_rr RAX RDX), (3,Pmulq_r R11), (3,Pmovq_rr RDX RAX), (1,Ppopl RAX)]"
+    using d0 d0_1 d4_1 d4_2 d6 d7 d9 d10 d12 d13 d16 d15 by auto
+  have c14_1:"exec_instr (snd(?xins!0)) (of_nat(fst(?xins!0))) xpc xrs xm = Next xpc1 xrs1 m1\<and>
+    exec_instr (snd(?xins!1)) (of_nat(fst(?xins!1))) xpc1 xrs1 m1 = Next xpc2 xrs2 m2 \<and>
+    exec_instr (snd(?xins!2)) (of_nat(fst(?xins!2))) xpc2 xrs2 m2 = Next xpc3 xrs3 m3 \<and>
+    exec_instr (snd(?xins!3)) (of_nat(fst(?xins!3))) xpc3 xrs3 m3 = Next xpc4 xrs4 m4 \<and>
+    exec_instr (snd(?xins!4)) (of_nat(fst(?xins!4))) xpc4 xrs4 m4 = Next xpc5 xrs5 m5 \<and> 
+    exec_instr (snd(?xins!5)) (of_nat(fst(?xins!5))) xpc5 xrs5 m5 = st6 " 
+    using b3 b4 b5 b6 b7 b8_1 by simp
+    
+  have b8_2:"st6\<noteq> Stuck" using mulq_subgoal_rr_aux4 c13 c14_1 by fast
+  hence "\<exists> xpc6 xrs6 m6. st6 = Next xpc6 xrs6 m6 "by (meson outcome.exhaust)
+  then obtain xpc6 xrs6 m6 where b8:"Next xpc6 xrs6 m6 = exec_instr xins6 (of_nat sz6) xpc5 xrs5 m5" using b8_1 by auto
 
-  have b4:"m3=m4" using  a0 exec_instr_def a4 by simp
-  have c4:"xrs3 RSP = xrs4 RSP" using a0 exec_instr_def a4 by auto
+  have c14:"exec_instr (snd(?xins!0)) (of_nat(fst(?xins!0))) xpc xrs xm = Next xpc1 xrs1 m1\<and>
+    exec_instr (snd(?xins!1)) (of_nat(fst(?xins!1))) xpc1 xrs1 m1 = Next xpc2 xrs2 m2 \<and>
+    exec_instr (snd(?xins!2)) (of_nat(fst(?xins!2))) xpc2 xrs2 m2 = Next xpc3 xrs3 m3 \<and>
+    exec_instr (snd(?xins!3)) (of_nat(fst(?xins!3))) xpc3 xrs3 m3 = Next xpc4 xrs4 m4 \<and>
+    exec_instr (snd(?xins!4)) (of_nat(fst(?xins!4))) xpc4 xrs4 m4 = Next xpc5 xrs5 m5 \<and> 
+    exec_instr (snd(?xins!5)) (of_nat(fst(?xins!5))) xpc5 xrs5 m5 = Next xpc6 xrs6 m6 " 
+    using c14_1 b8 by simp
+    
+  
+  let "?st'" = "x64_sem (fst (x64_prog!(unat pc))) ?l_bin xst" 
+  have c16:"snd (snd (x64_prog!(unat pc))) = ?l_bin" using a6 c0 a5 aux5 by metis
+  have "x64_prog!(unat pc) = the (per_jit_ins ?bpf_ins)" using aux5 a5 a6 by blast
+  then have c5:"x64_prog!(unat pc) = the (per_jit_mul_reg64 dst src)" using b2 False by simp
+  have c17:"(fst (x64_prog!(unat pc))) = length ?xins" using per_jit_mul_reg64_def c2
+      apply(cases "(bpf_to_x64_reg dst)",simp_all) using c5 by force
+   have c15:"(fst (x64_prog!(unat pc))) = (Suc(Suc(Suc(Suc(Suc(Suc 0))))))" using c17 by simp
+  (*let "?st'" = "x64_sem (Suc(Suc(Suc(Suc(Suc(Suc 0)))))) ?l_bin xst" *)
+   (*have cn:"?st' = Next xpc6 xrs6 m6" using c15 b3 b4 b5 b6 b7 b8  d3_0 d4_0 d5_1 d8_1 d11_1 d14_1 sorry*)
+   have c3_1:"x64_decode (unat xpc) ?l_bin \<noteq> None" using a7 using d3_0 by simp
+   hence c3_2:"?st' = (case x64_decode (unat xpc) ?l_bin of
+                  None \<Rightarrow> Stuck |
+                 Some (sz, ins) \<Rightarrow>
+              x64_sem (Suc(Suc(Suc(Suc(Suc 0))))) ?l_bin (exec_instr ins (of_nat sz) xpc xrs xm))" 
+      using a3 c0_1 c15 c0 d3_0 apply(cases xst,simp_all) 
+      apply(cases "prog ! unat pc",simp_all)
+      subgoal for x91 by(cases "x64_decode (unat xpc) ?l_bin",simp_all)
+      done
+    have c3:"?st' = x64_sem (Suc(Suc(Suc(Suc(Suc 0))))) ?l_bin (Next xpc1 xrs1 m1)" 
+      using c3_1 c3_2 d3_0 b3 by (simp add: a7)
 
-  have b5:"m4=m5" using a0 exec_instr_def a5 by simp
-  have c5:"xrs4 RSP = xrs5 RSP" using a0 exec_instr_def a5 by auto
+    have c4_0:"xpc1 = of_nat (length ?l_bin1)" using d0_1 a7 b3 exec_instr_def by(cases xins1,simp_all)
+    have c4_4:"unat xpc1 = of_nat (0+length ?l_bin1)" using d3_0 of_nat_def c4_0 by simp
+    hence c4_1:"x64_decode (unat xpc1) ?l_bin \<noteq> None" using d4_0 a7 by simp     
+    have c4_2:"?st' = (case x64_decode (unat xpc1) ?l_bin of
+                  None \<Rightarrow> Stuck |
+                 Some (sz, ins) \<Rightarrow>
+              x64_sem (Suc(Suc(Suc(Suc 0)))) ?l_bin (exec_instr ins (of_nat sz) xpc1 xrs1 m1))" 
+      using c3 a3 c0_1 c15 c0 c3_1 apply(cases "Next xpc1 xrs1 m1",simp_all) 
+      apply(cases "prog ! unat pc",simp_all)
+      subgoal for x91 by(cases "x64_decode (unat xpc1) ?l_bin",simp_all)
+      done
+    
+    have c4:"?st' = x64_sem (Suc(Suc(Suc(Suc 0)))) ?l_bin (Next xpc2 xrs2 m2)" 
+      using c4_2 d4_0 c4_4 b4 by simp  
 
-  have b5_1:"Next xpc6 xrs6 m6 = exec_pop xpc5 1 M64 m5 xrs5 RAX" using a6 a0 exec_instr_def by simp
-  have b5_2:"Mem.loadv M64 m5 ?addr \<noteq> None" using store_load_consistency b2 b3 b4 b5 by blast
-  have b5_3:"Mem.loadv M64 m5 ?addr = Some (Vlong (xrs1 RAX))" using b2 b3 b4 b5 store_load_consistency by auto
-  have b5:"m6 = m5 \<and> xrs6 RSP = xrs RSP" using exec_pop_def b5_2
-    apply(cases "Mem.loadv M64 m5 ?addr",simp_all) 
-     apply(cases "Vlong (xrs1 RAX)",simp_all)
-    subgoal for a x5 
-      using b5_1 b5_3 c2 c3 c4 c5 c1 by force
-    done
-  have d5:"xrs6 RAX = xrs RAX" using exec_pop_def b5_2
-    apply(cases "Mem.loadv M64 m5 ?addr",simp_all) 
-     apply(cases "Vlong (xrs1 RAX)",simp_all)
-    subgoal for a x5 
-      using b5_1 b5_3 c2 c3 c4 c5 d1 d2 by force
-    done
-  thus ?thesis using d5 b5 by simp
-qed
-
-lemma mulq_subgoal_rr_aux1_4:
-  "xins = [(3,Pmovq_rr R11 (bpf_to_x64_reg src)), (1,Ppushl_r RAX), (3,Pmovq_rr RAX RDX), (3,Pmulq_r R11), (3,Pmovq_rr RDX RAX), (1,Ppopl RAX)] \<Longrightarrow>
-    exec_instr (snd(xins!0)) (of_nat(fst(xins!0))) pc rs xm = Next pc1 rs1 m1\<and>
-    exec_instr (snd(xins!1)) (of_nat(fst(xins!1))) pc1 rs1 m1 = Next pc2 rs2 m2 \<and>
-    exec_instr (snd(xins!2)) (of_nat(fst(xins!2))) pc2 rs2 m2 = Next pc3 rs3 m3 \<and>
-    exec_instr (snd(xins!3)) (of_nat(fst(xins!3))) pc3 rs3 m3 = Next pc4 rs4 m4 \<and>
-    exec_instr (snd(xins!4)) (of_nat(fst(xins!4))) pc4 rs4 m4 = Next pc5 rs5 m5 \<and> 
-    exec_instr (snd(xins!5)) (of_nat(fst(xins!5))) pc5 rs5 m5 = Next pc6 rs6 m6 \<Longrightarrow>
-  \<forall> r. bpf_to_x64_reg r \<notin> {RDX} \<longrightarrow> rs (bpf_to_x64_reg r) = rs6 (bpf_to_x64_reg r) "
-  using mulq_subgoal_rr_aux1_3 mulq_subgoal_rr_aux1_1 reg_r11_consist reg_rsp_consist 
-  by (smt (z3) insert_iff)
-
-
-lemma mulq_subgoal_rr_aux2_1:
-  "xins = Pmulq_r (bpf_to_x64_reg src) \<Longrightarrow> 
-  Next pc' reg' m' = exec_instr xins sz pc reg m \<Longrightarrow>
-  \<forall> r. r \<notin> {RAX, RDX} \<longrightarrow> reg' r = reg r"
-  by (simp add: exec_instr_def)
-
-
-lemma mulq_subgoal_rr_aux3:"bins = BPF_ALU64 BPF_MUL dst (SOReg src) \<Longrightarrow> 
-  sbpf_step prog (SBPF_OK pc rs m) = (SBPF_OK pc' rs' m') \<Longrightarrow> 
-  prog!(unat pc) = bins \<Longrightarrow>
-  \<forall> r \<noteq> dst. rs' r = rs r"
-  apply(cases bins,simp_all)
-  apply(cases "prog ! unat pc", simp_all)
-  subgoal for x91 apply(simp split:if_split_asm) 
-    apply(unfold eval_alu_def eval_reg_def,simp_all)
-    by auto
-  done
-
-lemma stack_is_not_changed_by_add:"Next spc' reg' m' = exec_instr xins sz spc reg m \<Longrightarrow> xins = Paddq_rr (bpf_to_x64_reg dst) (bpf_to_x64_reg src) 
-   \<Longrightarrow> match_stack reg m \<Longrightarrow> match_stack reg' m'"
-proof-
-  assume a0:"Next spc' reg' m' = exec_instr xins sz spc reg m" and
-  a1:"xins = Paddq_rr (bpf_to_x64_reg dst) (bpf_to_x64_reg src) " and
-  a2:"match_stack reg m"
-  have b0:"bpf_to_x64_reg dst \<noteq> RSP" using bpf_to_x64_reg_def by (cases dst,simp_all)
-  have b1:"reg SP = reg' SP" using exec_instr_def a0 a1 exec_instr_def b0 by simp
-  have b2:"m = m'" using a0 a1 exec_instr_def by force
-  have "match_stack reg' m'" using b1 b2 a2 match_stack_def by auto
-  thus ?thesis by blast
-qed
-
-lemma mem_is_not_changed_by_add:"Next spc' reg' m' = exec_instr xins sz spc reg m \<Longrightarrow> xins = Paddq_rr (bpf_to_x64_reg dst) (bpf_to_x64_reg src) 
-   \<Longrightarrow> m = m'"
-  using exec_instr_def by simp
-
-lemma mem_is_not_changed_by_mov:"Next spc' reg' m' = exec_instr xins sz spc reg m \<Longrightarrow> xins = Pmovq_rr (bpf_to_x64_reg dst) (bpf_to_x64_reg src) 
-   \<Longrightarrow> m = m'"
-  using exec_instr_def by simp
-
-lemma mem_is_not_changed_by_mul:"Next spc' reg' m' = exec_instr xins sz spc reg m \<Longrightarrow> xins = Pmulq_r (bpf_to_x64_reg src) 
-   \<Longrightarrow> m = m'"
-  using exec_instr_def by simp
-
-lemma mem_is_not_changed:"s2 = sbpf_step prog s1 \<Longrightarrow> s1 = (SBPF_OK pc1 rs1 m1) \<Longrightarrow> s2 = (SBPF_OK pc2 rs2 m2) \<Longrightarrow> m1 = m2"
-  apply(cases "prog!(unat pc1)", simp_all)
-  subgoal for x11 x12 x13 
-    by (metis bpf_instruction.simps(361) sbpf_state.simps(6))
-  subgoal for x21 x22 x23 x24
-    by (metis bpf_instruction.simps(362) sbpf_state.simps(6))
-  subgoal for x31 x32 x33 x34 
-    by (metis bpf_instruction.simps(363) sbpf_state.simps(6))
-  subgoal for x4 
-    by (metis bpf_instruction.simps(364) sbpf_state.distinct(3))
-  subgoal for x51 x52 x53 
-    by (metis bpf_instruction.simps(365) sbpf_state.simps(6))
-  subgoal for x6 
-    by (metis bpf_instruction.simps(366) sbpf_state.simps(6))
-  subgoal for x71 x72
-    by (metis bpf_instruction.simps(367) sbpf_state.simps(6))
-  subgoal for x81 x82
-    by (metis bpf_instruction.simps(368) sbpf_state.simps(6))
-  subgoal for x91 x92 x93
-    apply(split if_splits, simp_all)
-    apply(split if_splits, simp_all)
-    apply(cases x91, simp_all)
-     apply(cases "eval_alu BPF_ADD x92 x93 rs1", simp_all)
-    apply(cases "eval_alu BPF_MUL x92 x93 rs1",simp_all)
-    done
-  subgoal for x10
-    by (metis bpf_instruction.simps(370) sbpf_state.simps(6))
-  subgoal for x111 x112
-    by (metis bpf_instruction.simps(371) sbpf_state.simps(6))
-  subgoal for x121 x122 x123
-    by (metis bpf_instruction.simps(372) sbpf_state.simps(6))
-  subgoal for x131 x132 x133
-    by (metis bpf_instruction.simps(373) sbpf_state.simps(6))
-  subgoal for x141 x142 x143
-    by (metis bpf_instruction.simps(374) sbpf_state.simps(6))
-  subgoal for x15
-    by (metis bpf_instruction.simps(375) sbpf_state.simps(6))
-  subgoal for x161 x162 x163 x164
-    by (metis bpf_instruction.simps(376) sbpf_state.simps(6))
-  subgoal for x171 x172
-    by (metis bpf_instruction.simps(377) sbpf_state.simps(6))
-  subgoal for x181 x182
-    by (metis bpf_instruction.simps(378) sbpf_state.simps(6))
-  by (metis (no_types, lifting) bpf_instruction.simps(379) sbpf_state.distinct(1) sbpf_state.simps(6))             
-
-(*lemma mem_is_not_changed2:"x64_sem 1 l xst1 = xst2 \<Longrightarrow> xst1 = Next xpc1 xrs1 m1 \<Longrightarrow> xst2 = Next xpc2 xrs2 m2 \<Longrightarrow> m1 = m2"
-  apply(cases "x64_decode (unat xpc1) l", simp_all)
-  subgoal for a apply(cases a, simp_all)
-    subgoal for aa b
-      apply(unfold exec_instr_def)
-      apply (cases b, simp_all)
-      apply(unfold exec_ret_def Let_def) 
-      apply(cases "loadv M64 m1 (xrs1 SP + u64_of_memory_chunk M64)", simp_all)
-      subgoal for ab apply(cases ab, simp_all)
+    have c5_1:"xpc2 = xpc1 + of_nat(length ?l_bin2)" using b4 d4_1 d4_2
+      apply(unfold exec_instr_def,simp_all)
+      apply(cases xins2,simp_all)
+      apply(unfold exec_push_def)
+      apply(cases "storev M64 m1 (Vptr 1 (xrs1 SP - u64_of_memory_chunk M64)) (Vlong (xrs1 RAX))",simp_all)
+       apply (metis One_nat_def of_nat_1 outcome.simps(3))
+      subgoal for a
+        by (metis d4_2 of_nat_1 outcome.inject)
+      done
+    have c5_2:"xpc2 = of_nat(length ?l_bin1+length ?l_bin2)" using c5_1 c4_0 by simp
+    have "length ?l_bin1+length ?l_bin2 = 4" using f0 f1 by simp 
+    hence c5_3:"unat xpc2 = (0 + length ?l_bin1+length ?l_bin2)" using c5_2 of_nat_def by auto
+    have "\<exists> tempst'. x64_sem (Suc 0) ?l_bin (Next xpc2 xrs2 m2) = tempst' \<and>
+    x64_sem (Suc(Suc(Suc 0))) ?l_bin tempst' = ?st'" using c4 x64_sem_add 
+      using One_nat_def plus_1_eq_Suc by presburger
+    then obtain tempst' where c5_4:"x64_sem (Suc 0) ?l_bin (Next xpc2 xrs2 m2) = tempst' \<and>
+    x64_sem (Suc(Suc(Suc 0))) ?l_bin tempst' = ?st'" by auto
+    have c5_5:"x64_decode (unat xpc2) ?l_bin \<noteq> None" using c5_3 d5_1 by simp
+    have c5_6:"x64_sem (Suc 0) ?l_bin (Next xpc2 xrs2 m2) = tempst'" using c5_4 by auto
+    have c5_7:"x64_decode (0 + length ?l_bin1+length ?l_bin2) ?l_bin = Some (sz3,xins3)" using d5_1 by simp
+    have "tempst' =  (case x64_decode (0 + length ?l_bin1+length ?l_bin2) ?l_bin of
+      None \<Rightarrow> Stuck |
+      Some (sz, ins) \<Rightarrow>
+        x64_sem 0 ?l_bin (exec_instr ins (of_nat sz) xpc2 xrs2 m2))" using c5_3 c5_6
+      by (metis x64_sem.simps(3))
+    hence "tempst' = x64_sem 0 ?l_bin (exec_instr xins3 (of_nat sz3) xpc2 xrs2 m2)" using c5_7 d5_1 c0_1 
+      apply(cases "x64_decode (0 + length ?l_bin1+length ?l_bin2) ?l_bin",simp_all)
+      subgoal for a apply(cases "prog ! unat pc",simp_all) 
+        subgoal for x91 by auto
         done
-    done
-  done
-  done*)
+      done
+    hence c5:"tempst' = Next xpc3 xrs3 m3" using b5 by simp
 
-lemma addq_subgoal_rr_generic:
-  assumes a0:"bins = BPF_ALU64 BPF_ADD dst (SOReg src)" and
-       a1:"per_jit_add_reg64_1 dst src = Some (n, off, l_bin)" and
-       a3:"x64_decode 0 l_bin = Some (length l_bin, xins)" and
-       a4:"sbpf_step prog (SBPF_OK pc rs m) = (SBPF_OK pc' rs' m')" and
-       a5:"Next spc' reg' xm' = exec_instr xins sz spc reg xm" and
-       a6:"match_state (SBPF_OK pc rs m) (Next spc reg xm) " and
-       a7:"prog!(unat pc) = bins"
-  shows "match_state (SBPF_OK pc' rs' m') (Next spc' reg' xm') "
-proof -
-    have b0:"xins = Paddq_rr (bpf_to_x64_reg dst) (bpf_to_x64_reg src)" 
-      using x64_encode_decode_consistency per_jit_add_reg64_1_def a1 a3 list_in_list_prop
-    by (smt (verit, ccfv_SIG) Pair_inject map_option_eq_Some option.inject)
-    moreover have b1:"(\<forall> r. (rs r) = reg (bpf_to_x64_reg r))" using a6 spec match_state_def match_reg_def by simp
-    moreover have b2:"(rs src) = reg (bpf_to_x64_reg src)" using a6 spec b1 by simp
-    hence b3:"(rs' dst) = reg' (bpf_to_x64_reg dst)" using aluq_subgoal_rr_aux1 b0 b1 b2 a0 a4 a5 a7 by metis
-    have b4:"\<forall> r \<noteq> dst. reg'(bpf_to_x64_reg r) = reg (bpf_to_x64_reg r)" using b0 a5 aluq_subgoal_rr_aux2 by blast
-    have b5:"\<forall> r \<noteq> dst. (rs' r) = (rs r)" using aluq_subgoal_rr_aux3 a0 a4 a7 by force
-    have b6:"\<forall> r \<noteq> dst. (rs r) = reg ((bpf_to_x64_reg r))" using a6 using b1 by blast
-    have b7:"(\<forall> r \<noteq> dst. (rs' r) = reg' ((bpf_to_x64_reg r)))" using b1 b4 b5 by presburger
-    have b8:"match_stack reg' xm'" using stack_is_not_changed_by_add a6 match_state_def a5 b0 by simp
-    have b9:"match_mem m' xm'" using mem_is_not_changed mem_is_not_changed_by_add match_state_def a6
-      by (metis (no_types, lifting) a4 a5 b0 outcome.simps(4) sbpf_state.simps(9))
-    thus ?thesis using b3 b7 match_state_def b8 b9 match_reg_def by fastforce
-  qed
-      
+    have c6_0:" x64_sem (Suc(Suc(Suc 0))) ?l_bin tempst' = ?st'" using c5_4 by auto
+    have c6_1:"xpc3 =  xpc2 + of_nat(length ?l_bin3)" using  b5 d6 
+      by(unfold exec_instr_def,simp_all)
+    have c6_2:"xpc3 = of_nat(length ?l_bin1+length ?l_bin2+length ?l_bin3)" using c6_1 c5_2 by auto
+    have "length ?l_bin1+length ?l_bin2+length ?l_bin3=7" using f0 f1 f2 by linarith
+    hence c6_3:"unat xpc3 = (0 + length ?l_bin1+length ?l_bin2+length ?l_bin3)" using c6_2 of_nat_def by auto
+    have "\<exists> tempst'. x64_sem (Suc 0) ?l_bin (Next xpc3 xrs3 m3) = tempst' \<and>
+    x64_sem ((Suc(Suc 0)))?l_bin tempst' = ?st'" using c4 x64_sem_add 
+      using One_nat_def plus_1_eq_Suc c5 c6_0 by presburger
+    then obtain tempst' where c6_4:"x64_sem (Suc 0) ?l_bin (Next xpc3 xrs3 m3) = tempst' \<and>
+    x64_sem ((Suc(Suc 0))) ?l_bin tempst' = ?st'" by auto
+    have c6_5:"x64_decode (unat xpc3) ?l_bin \<noteq> None" using c6_3 d8_1 by simp
+    have c6_6:"x64_sem (Suc 0) ?l_bin (Next xpc3 xrs3 m3) = tempst'" using c6_4 by auto
+    have "tempst' =  (case x64_decode (0 + length ?l_bin1+length ?l_bin2+length ?l_bin3) ?l_bin of
+      None \<Rightarrow> Stuck |
+      Some (sz, ins) \<Rightarrow>
+        x64_sem 0 ?l_bin (exec_instr ins (of_nat sz) xpc3 xrs3 m3))" using c6_3 c6_6
+      by (metis x64_sem.simps(3))
+    hence "tempst' = x64_sem 0 ?l_bin (exec_instr xins4 (of_nat sz4) xpc3 xrs3 m3)" using  d8_1 c6_5
+      by(cases "x64_decode (0 + length ?l_bin1+length ?l_bin2) ?l_bin",simp_all)
+    hence c6:"tempst' = Next xpc4 xrs4 m4" using b6 by simp
 
-lemma exit_subgoal_rr_generic:
-  assumes a0:"bins = BPF_EXIT" and
-       a1:"per_jit_exit = Some (n, off, l_bin)" and
-       a3:"x64_decode 0 l_bin = Some (n, xins)" and
-       a4:"sbpf_step prog (SBPF_OK pc rs m) = st'" and
-       a5:"xst' = exec_instr xins sz spc reg m" and
-       a6:"match_state (SBPF_OK pc rs m) (Next spc reg m) " and
-       a7:"prog!(unat pc) = bins" and
-       a8:"prog \<noteq> [] \<and> unat pc < length prog \<and> unat pc \<ge> 0"
-     shows "match_state st' xst'"
-proof-
-  have b0:"st' = SBPF_Success (rs BR0)" using a0 a4 a7 a8 by simp
-  have b1:"xins = Pret" using x64_encode_decode_consistency per_jit_exit_def a0 a1 a3 list_in_list_prop
-    by (smt (verit, ccfv_SIG) map_option_eq_Some option.inject prod.inject)
-  moreover have b2:"(\<forall> r. (rs r) = reg (bpf_to_x64_reg r))" using a6 spec match_state_def match_reg_def by simp
-  moreover have b3:"(rs BR0) = reg (bpf_to_x64_reg BR0)" using a6 spec b2 by simp
-  (*have b4:"Mem.loadv M64 m ((reg SP) + (u64_of_memory_chunk M64)) \<noteq> None" using match_state_def a6 match_stack_def by auto
-  hence "\<exists> x. Mem.loadv M64 m ((reg SP) + (u64_of_memory_chunk M64)) = x \<and> x\<noteq> None" by simp
-  hence "\<exists> v. Mem.loadv M64 m ((reg SP) + (u64_of_memory_chunk M64)) = Some v" by simp*)
-  hence b5_1:"\<exists> v. Mem.loadv M64 m ((reg SP) + (u64_of_memory_chunk M64)) = Some (Vlong v)" using match_state_def a6 match_stack_def by auto
-  obtain v where b5_2:"Mem.loadv M64 m ((reg SP) + (u64_of_memory_chunk M64)) = Some (Vlong v)" using b5_1 by blast
-  let "?reg'" = "(reg#SP <- ((reg SP) + (u64_of_memory_chunk M64)))"
-  have b5_3:"xst' = Next v ?reg' m" using exec_instr_def exec_ret_def a5 b1 b5_2 by simp
-  hence b5:"?reg' (bpf_to_x64_reg BR0) = reg (bpf_to_x64_reg BR0)" by (simp add: bpf_to_x64_reg_def)
-  thus ?thesis using exec_instr_def b3 b1 b0 a5 using b5_2 exec_ret_def match_state_def by force
-qed
+    have c7_0:" x64_sem (Suc(Suc 0)) ?l_bin tempst' = ?st'" using c6_4 by auto
+    have c7_1:"xpc4 =  xpc3 + of_nat(length ?l_bin3)" using b6 d9
+      by(unfold exec_instr_def,simp_all)
+    hence c7_2:"xpc4 = of_nat(length ?l_bin1+length ?l_bin2+length ?l_bin3+length ?l_bin4)" using c6_2 by auto
+    have "length ?l_bin1+length ?l_bin2+length ?l_bin3+length ?l_bin4 = 10" using f0 f1 f2 f3 by simp
+    hence c7_3:"unat xpc4 = (0 + length ?l_bin1+length ?l_bin2+length ?l_bin3+length ?l_bin4)" using of_nat_def c7_2 by auto
+    have "\<exists> tempst'. x64_sem (Suc 0) ?l_bin (Next xpc4 xrs4 m4) = tempst' \<and>
+    x64_sem (Suc 0) ?l_bin tempst' = ?st'" using x64_sem_add 
+      using One_nat_def plus_1_eq_Suc c6 c7_0 by presburger
+    then obtain tempst' where c7_4:"x64_sem (Suc 0) ?l_bin (Next xpc4 xrs4 m4) = tempst' \<and>
+    x64_sem (Suc 0) ?l_bin tempst' = ?st'" by auto
+    have c7_5:"x64_decode (unat xpc4) ?l_bin \<noteq> None" using c7_3 d11_1 by simp
+    have c7_6:"x64_sem (Suc 0) ?l_bin (Next xpc4 xrs4 m4) = tempst'" using c7_4 by auto
+    have "tempst' =  (case x64_decode (0 + length ?l_bin1+length ?l_bin2+length ?l_bin3+length ?l_bin4) ?l_bin of
+      None \<Rightarrow> Stuck |
+      Some (sz, ins) \<Rightarrow>
+        x64_sem 0 ?l_bin (exec_instr ins (of_nat sz) xpc4 xrs4 m4))" using c7_3 c7_6
+      by (metis x64_sem.simps(3))
+    hence "tempst' = x64_sem 0 ?l_bin (exec_instr xins5 (of_nat sz5) xpc4 xrs4 m4)" using d11_1
+      by(cases "x64_decode (0 + length ?l_bin1+length ?l_bin2) ?l_bin",simp_all)
+    hence c7:"tempst' = Next xpc5 xrs5 m5" using b7 by simp
 
+    have c8_0:" x64_sem (Suc 0) ?l_bin tempst' = ?st'" using c7_4 by auto
+    have c8_1:"xpc5 =  xpc4 + of_nat(length ?l_bin5)" using b7 d12
+      by(unfold exec_instr_def,simp_all)
+    hence c8_2:"xpc5 = of_nat(length ?l_bin1+length ?l_bin2+length ?l_bin3+length ?l_bin4+length ?l_bin5)" using c7_2 by auto
+    have "length ?l_bin1+length ?l_bin2+length ?l_bin3+length ?l_bin4+length ?l_bin5 = 13" using  f0 f1 f2 f3 f4 by simp
+    hence c8_3:"unat xpc5 = (0 + length ?l_bin1+length ?l_bin2+length ?l_bin3+length ?l_bin4+length ?l_bin5)" using of_nat_def c8_2 by auto
+    have "\<exists> tempst'. x64_sem (Suc 0) ?l_bin (Next xpc5 xrs5 m5) = tempst' \<and>
+    x64_sem 0 ?l_bin tempst' = ?st'" using x64_sem_add 
+      using One_nat_def plus_1_eq_Suc c7 c8_0 by auto
+    then obtain tempst' where c8_4:"x64_sem (Suc 0) ?l_bin (Next xpc5 xrs5 m5) = tempst' \<and>
+    x64_sem 0 ?l_bin tempst' = ?st'" by auto
+    have c8_5:"x64_decode (unat xpc5) ?l_bin \<noteq> None" using c8_3 d14_1 by simp
+    have c8_6:"x64_sem (Suc 0) ?l_bin (Next xpc5 xrs5 m5) = tempst'" using c8_4 by auto
+    have "tempst' =  (case x64_decode (0 + length ?l_bin1+length ?l_bin2+length ?l_bin3+length ?l_bin4+length ?l_bin5) ?l_bin of
+      None \<Rightarrow> Stuck |
+      Some (sz, ins) \<Rightarrow>
+        x64_sem 0 ?l_bin (exec_instr ins (of_nat sz) xpc5 xrs5 m5))" using c8_3 c8_6
+      by (metis x64_sem.simps(3))
+    hence "tempst' = x64_sem 0 ?l_bin (exec_instr xins6 (of_nat sz6) xpc5 xrs5 m5)" using d14_1 
+      by(cases "x64_decode (0 + length ?l_bin1+length ?l_bin2) ?l_bin",simp_all)
+    hence c8:"tempst' = Next xpc6 xrs6 m6" using b8 by simp
+    have cn:"?st' = Next xpc6 xrs6 m6" using c8 c8_4 by simp
 
-(*
-    Some l_bin = x64_encodes2 ins \<Longrightarrow>
-    x64_decodes_aux (length ins) 0 l_bin = Some ins_list \<Longrightarrow>
-    map snd ins_list = ins"
-*)
-
-
-lemma aux1:"length prog \<noteq> 0 \<and> unat pc < length prog \<and> unat pc \<ge> 0 \<Longrightarrow> 
-  s' = sbpf_step prog s \<Longrightarrow>
-  s = (SBPF_OK pc rs m) \<Longrightarrow> 
-  s' = (SBPF_OK pc' rs' m') \<Longrightarrow> 
-  \<exists> dst src. prog!(unat pc) = BPF_ALU64 BPF_ADD dst (SOReg src) \<or> prog!(unat pc) = BPF_ALU64 BPF_MUL dst (SOReg src)"
-  apply(cases "prog!(unat pc)",simp_all)
-  subgoal for x91 x92 x93 
-   apply(unfold eval_alu_def Let_def)
-    apply(cases x91,simp_all) 
-     apply(cases x93, simp_all)
-     apply(cases x93, simp_all)
-    done
-  done
-
-lemma aux2:"length prog \<noteq> 0 \<and> unat pc < length prog \<and> unat pc \<ge> 0 \<Longrightarrow> 
-  s' = sbpf_step prog s \<Longrightarrow>
-  s = (SBPF_OK pc rs m) \<Longrightarrow> 
-  s' \<noteq> SBPF_Err \<Longrightarrow> 
-  \<exists> dst src. prog!(unat pc) \<in> {BPF_ALU64 BPF_ADD dst (SOReg src),BPF_EXIT, BPF_ALU64 BPF_MUL dst (SOReg src)}"
-  apply(cases "prog!(unat pc)",simp_all)
-  subgoal for x91 x92 x93 
-   apply(unfold eval_alu_def Let_def)
-    apply(cases x91,simp_all) 
-     apply(cases x93, simp_all)
-    apply(cases x93, simp_all)
-    done
-  done
-
-
-lemma aux3:"jitper prog = Some x64_prog \<Longrightarrow> length x64_prog = length prog"
-proof (induction prog arbitrary: x64_prog)
-  case Nil
-  then show ?case by simp
+  have e1:"(\<forall> r. (rs r) = xrs (bpf_to_x64_reg r))" using a1 spec match_state_def match_reg_def a4 a3 by simp
+  moreover have e2:"(rs src) = xrs (bpf_to_x64_reg src)" using spec e1 by simp
+  moreover have e2_1:"(rs dst) = xrs (bpf_to_x64_reg dst)" using spec e1 by simp
+  hence e3:"(rs' dst) = xrs6 (bpf_to_x64_reg dst)"            
+    using mulq_subgoal_rr_aux1_2 c2 c0_1 a0 a1 a2 a3 e2 e2_1 c14 c13 by fastforce
+  have " \<forall> r. bpf_to_x64_reg r \<notin> {RDX}\<longrightarrow> xrs6 (bpf_to_x64_reg r) = xrs (bpf_to_x64_reg r)" 
+    using c13 c14 mulq_subgoal_rr_aux1_4 c2 bpf_to_x64_reg_corr by fastforce
+  hence e4:" \<forall> r\<noteq>dst. xrs6 (bpf_to_x64_reg r) = xrs (bpf_to_x64_reg r)" 
+    using bpf_to_x64_reg_corr bpf_to_x64_reg_corr2 c2  by (metis singletonD)
+  have e5:"\<forall> r \<noteq> dst. (rs' r) = (rs r)" using mulq_subgoal_rr_aux3 a0 a1 a2 c0_1 by blast
+  have e7:"(\<forall> r \<noteq> dst. (rs' r) = xrs6 ((bpf_to_x64_reg r)))" using e1 e4 e5 by presburger
+  have e8:"match_stack xrs6 m6" using mulq_match_stack match_state_def a4 c13 c14 a3 a1 by auto
+  have e9:"match_mem m' m6" using mulq_match_mem match_state_def a4 c13 c14 a3 a1 a0 a1 a2 c0_1 by fastforce
+  have "match_state s' ?st'" using e3 e7 match_state_def e8 e9 match_reg_def cn a2 by fastforce
+  thus ?thesis using c16 by simp
 next
-  case (Cons h xs)
-  assume "jitper (h # xs) = Some x64_prog"
-  then have a0:"\<exists> x. per_jit_ins h = Some x" using Cons(1) by (cases "per_jit_ins h"; auto)
-  obtain x where a1:"per_jit_ins h = Some x" using a0 by auto
-  then have a2:"\<exists> res. jitper xs = Some res" using Cons(1) apply (cases "jitper xs"; auto) 
-    using Cons.prems(1) by force
-  obtain res where a3:"jitper xs = Some res" using a2 by auto
-  have a4:" x64_prog = x # res" using Cons(1) a3 a1
-    using Cons.prems(1) by force
-  then have a5:"length ( x64_prog) = length (h # xs)" using a4 Cons.IH a3 by fastforce
-  then show ?case using Cons by simp
-qed
-
-
-value "[2::nat,3]!(unat (0::u64))"
-
-
-lemma aux5:"jitper prog = Some x64_prog \<Longrightarrow> unat pc \<ge> 0 \<and> unat pc < length prog \<Longrightarrow> 
-  prog!(unat pc) = bins \<Longrightarrow> x64_prog!(unat pc) = l_bin \<Longrightarrow> prog \<noteq> [] 
-  \<Longrightarrow> l_bin = the (per_jit_ins bins)"
-proof (induction prog arbitrary: x64_prog pc bins l_bin)
-  case Nil
-  then show ?case by simp
-next
-  case (Cons a prog)
-  then show ?case
-  proof-
-    have a0:"unat pc = 0 \<or> unat pc \<ge> 1" by auto
-    show ?thesis
-    proof (cases "unat pc = 0")
+  case False
+    have c2_1:"(bpf_to_x64_reg dst) = RAX \<or> (bpf_to_x64_reg dst) \<notin> {RAX, RDX}" using c2_0 False by blast
+    thus ?thesis
+    proof (cases "(bpf_to_x64_reg dst) = RAX")
       case True
-      have "unat pc = 0" using True a0 by simp
-      have b0:"\<exists> x. per_jit_ins a = Some x" using Cons by (cases "per_jit_ins a"; auto)
-      obtain x where b1:"per_jit_ins a = Some x" using b0 by auto
-      then have b2:"\<exists> res. jitper prog = Some res" using Cons(1) apply (cases "jitper prog"; auto) 
-        using Cons.prems(1) by force
-      obtain res where b3:"jitper prog = Some res" using b2 by auto
-      have b4:"x64_prog = x # res" using Cons(1) b3 b1 Cons by force
-      have bn:"l_bin = the (per_jit_ins bins)" using b1 b2 
-        using Cons.prems(3) Cons.prems(4) True b4 by fastforce
-      then show ?thesis using bn by blast
+      then show ?thesis sorry
     next
       case False
-      have "\<exists> res. jitper prog = Some res" using Cons 
-        apply (cases "jitper prog"; simp_all) 
-        apply(cases a, simp_all) 
-        subgoal for x91 x92 x93 apply(cases x91,simp_all) 
-           apply(cases x93,simp_all)
-          subgoal for x2 apply(cases "per_jit_add_reg64_1 x92 x2",simp_all) 
-            done 
-          apply(cases x93,simp_all)
-          subgoal for x2 apply(cases "per_jit_mul_reg64 x92 x2",simp_all)
-            done 
-          done
-        apply(unfold per_jit_exit_def) 
-        apply(cases per_jit_exit,simp_all) 
-        done
-      then obtain res where b0:"jitper prog = Some res" by auto
-      have b1:"\<exists> x. per_jit_ins a = Some x" using Cons by (cases "per_jit_ins a"; auto)
-      obtain x where b2:"per_jit_ins a = Some x" using b1 by auto
-      have c0:" Some (x # res) = Some x64_prog" using b0 b2 Cons by auto
-      have c1:"unat pc \<ge> 1" using a0 False by blast
-      have c2:"(a#prog) ! unat pc = bins" using c0 Cons.prems(3) by blast
-      let "?pc'" = "unat pc -1"
-      have c4:"0 \<le> ?pc' \<and> ?pc' < length prog \<and>
-      prog ! ?pc' = bins \<and> res ! ?pc' = l_bin \<and> prog \<noteq> []" using Cons.prems(2) Cons.prems(3) Cons.prems(4) c0 c1 by auto
-      (* have cn:"0 \<le> unat pc \<and> unat pc < length prog \<Longrightarrow> 
-          prog ! unat pc = bins \<Longrightarrow> ?x ! unat pc = l_bin \<Longrightarrow> Some (snd (snd l_bin)) = per_jit_ins bins" using Cons
-        by (metis (no_types, lifting) jit.simps(2) option.case_eq_if option.collapse)*)
-      have c5:"l_bin = the (per_jit_ins bins)" using c4 Cons 
-         False jitper.simps(2) order_neq_le_trans unat_gt_0 unat_minus_one
-        by (metis (no_types, lifting) b0)
-      then show ?thesis using c5 by blast
-    qed
-  qed
+      have "(bpf_to_x64_reg dst) \<notin> {RAX, RDX}" using c2_1 False by blast
+      then show ?thesis sorry
+    qed   
 qed
+qed
+qed
+
+lemma demo2_aux:
+  "\<lbrakk> sbpf_sem n prog s = s';
+   s = (SBPF_OK pc rs m);
+   s' = (SBPF_OK pc' rs' m');
+   xst = (Next xpc xrs xm);
+   match_state s xst;
+   jitper prog = Some x64_prog;
+   prog \<noteq> [];
+   xpc = 0;
+   x64_sem1 n pc x64_prog xst = xst' \<rbrakk> \<Longrightarrow>
+   match_state s' xst'"
+(* \<exists> xst'. x64_sem1 n pc x64_prog xst = xst' \<and> match_state s' xst'"*)
+proof (induction n arbitrary: prog s s' pc rs m pc' rs' m' xst' xst xpc xrs xm x64_prog xst')
+  case 0
+  then show ?case
+    by simp
+next
+  case (Suc n)
+  assume 
+       assm1: "sbpf_sem (Suc n) prog s = s'" and
+       assm2:"s = SBPF_OK pc rs m" and
+       assm3:"s' = SBPF_OK pc' rs' m'" and
+       assm4:"xst = Next xpc xrs xm" and
+       assm5:"match_state s xst" and
+       assm6:"jitper prog = Some x64_prog" and
+       assm7:"prog \<noteq> [] " and
+       assm8:"xpc = 0" and
+       assm9:"x64_sem1 (Suc n) pc x64_prog xst = xst'"
+  then obtain s1 where s1_eq: "s1 = sbpf_step prog s" by simp
+  have n_step_def:"sbpf_sem n prog s1 = s'" using s1_eq assm1 sbpf_sem_induct
+    by (metis sbpf_sem.simps(2))
+  have a0:"unat pc < length prog \<and> unat pc \<ge> 0" using assm1 assm3 
+    using Suc.prems(2) assm7 pc_scope_aux by blast
+  moreover have a1:"\<exists> pc1 rs1 m1. s1 = (SBPF_OK pc1 rs1 m1)"
+    by (metis Suc.prems(3) bot_nat_0.not_eq_extremum intermediate_step_is_ok n_step_def sbpf_sem.simps(1) sbpf_state.simps(6))
+  obtain pc1 rs1 m1 where a2:"s1 = (SBPF_OK pc1 rs1 m1)" using a1 by auto
+  have a3:"m1 = m" using mem_is_not_changed s1_eq assm2 a2 by blast
+  let "?num" = "(fst(x64_prog!(unat pc)))"
+  have "\<exists> xst1. x64_sem (fst(x64_prog!(unat pc))) (snd (snd ((x64_prog!(unat pc)))))(Next xpc xrs xm) = xst1 \<and> match_state s1 xst1"
+    using s1_eq assm2 a2 assm4 assm5 assm6 assm7 assm8 assm8 demo1 by (metis (mono_tags, lifting) calculation)
+  then obtain xst1 where a4:"x64_sem ?num (snd (snd ((x64_prog!(unat pc)))))(Next 0 xrs xm) = xst1 \<and> match_state s1 xst1" using assm8 by auto
+  hence a4_1:"x64_sem ?num (snd (snd ((x64_prog!(unat pc)))))(Next 0 xrs xm) = xst1" by auto
+  have an:"\<exists> xpc1 xrs1 xm1. xst1 = Next xpc1 xrs1 xm1" using a4 by (metis match_s_not_stuck outcome.exhaust)
+  then obtain xpc1 xrs1 xm1 where a10:"xst1 = Next xpc1 xrs1 xm1" by auto
+  let "?xst1" = "Next 0 xrs1 xm1"
+  have a5:"match_state s1 ?xst1" using an match_state_def
+    using a10 a2 a4 by fastforce
+  have "\<exists> num off l. x64_prog!(unat pc) = (num,off,l)" by (metis split_pairs)
+  then obtain num off l where a6:"x64_prog!(unat pc) = (num,off,l)" by auto
+  have a7:"l = (snd (snd ((x64_prog!(unat pc)))))" using a6 by simp
+  let "?pc" = "pc+off"
+  have a9:"x64_sem1 n ?pc x64_prog ?xst1 = xst'" using x64_sem1_induct_aux3 assm4 assm9 a7 a6 a4_1 a10 by (metis fst_conv)
+  have a13:"?pc = pc1" using corr_pc_aux2 assm6 a0 s1_eq a6 a2 assm7 assm2 by auto
+  from Suc.IH have " sbpf_sem n prog s = s' \<Longrightarrow>
+           s = SBPF_OK pc rs m \<Longrightarrow>
+           s' = SBPF_OK pc' rs' m' \<Longrightarrow>
+           xst = Next xpc xrs xm \<Longrightarrow>
+           match_state s xst \<Longrightarrow>
+           jitper prog = Some x64_prog \<Longrightarrow>
+           prog \<noteq> [] \<and> unat pc < length prog \<and> 0 \<le> unat pc \<Longrightarrow> 
+           xpc = 0 \<Longrightarrow> 
+           x64_sem1 n pc x64_prog xst = xst' \<Longrightarrow> 
+           match_state s' xst'" by blast
+  have "x64_sem1 n pc1 x64_prog (Next 0 xrs1 xm1) = xst' \<and> match_state s' xst'" using n_step_def a2 assm3 a10 a5 assm6 assm7 assm8 a9 Suc a13 by blast
+  hence an:"match_state s' xst'" by blast
+  then show ?case using an by auto
+qed
+
+
+lemma demo2:
+  "\<lbrakk> sbpf_sem n prog s = s';
+   s = (SBPF_OK pc rs m);
+   s' = (SBPF_OK pc' rs' m);
+   xst = (Next xpc xrs m);
+   match_state s xst;
+   jitper prog = Some x64_prog;
+   prog \<noteq> [] \<and> unat pc < length prog \<and> unat pc \<ge> 0;
+   xpc = 0 \<rbrakk> \<Longrightarrow>
+   \<exists> xst'. x64_sem1 n pc x64_prog xst = xst' \<and> match_state s' xst'"
+  using demo2_aux by blast
+
 
 
                                   
