theory/JITPer_add.thy
@@ -1,0 +1,97 @@
+theory JITPer_add
+imports
+  Main
+  rBPFCommType rBPFSyntax rBPFSem
+  x64Syntax x64Semantics x64Assembler
+  JITPer_aux
+
+begin
+
+lemma aluq_subgoal_rr_aux1:
+     "bins = BPF_ALU64 BPF_ADD dst (SOReg src) \<Longrightarrow>
+     xins = Paddq_rr (bpf_to_x64_reg dst) (bpf_to_x64_reg src) \<Longrightarrow>
+     prog!(unat pc) = bins \<Longrightarrow>
+     sbpf_step prog (SBPF_OK pc rs m) = (SBPF_OK pc' rs' m')  \<Longrightarrow>
+     Next spc' reg' xm' = exec_instr xins sz spc reg xm \<Longrightarrow>
+     reg (bpf_to_x64_reg dst) = rs dst \<Longrightarrow>
+     reg (bpf_to_x64_reg src) = rs src \<Longrightarrow>
+     reg' (bpf_to_x64_reg dst) = (rs' dst)"
+  apply (unfold exec_instr_def step)
+  apply simp
+  apply(cases "prog ! unat pc",simp_all)
+  subgoal for x91 apply(simp split:if_split_asm) 
+    apply(unfold eval_alu_def eval_reg_def,simp_all)
+    by auto
+  done
+
+
+lemma aluq_subgoal_rr_aux2_1:"xins = Paddq_rr dst src \<Longrightarrow> 
+  Next pc' reg' m' = exec_instr xins sz pc reg m \<Longrightarrow>
+  \<forall> r \<noteq> dst. reg' r = reg r"
+  by (simp add: exec_instr_def)
+
+
+lemma aluq_subgoal_rr_aux2:"xins = Paddq_rr (bpf_to_x64_reg dst) (bpf_to_x64_reg src) \<Longrightarrow> 
+  Next pc' reg' m' = exec_instr xins sz pc reg m \<Longrightarrow>
+  \<forall> r \<noteq> dst. reg' (bpf_to_x64_reg r) = reg (bpf_to_x64_reg r)"
+  using aluq_subgoal_rr_aux2_1 by simp
+
+
+
+lemma aluq_subgoal_rr_aux3:"bins = BPF_ALU64 BPF_ADD dst (SOReg src) \<Longrightarrow> 
+  sbpf_step prog (SBPF_OK pc rs m) = (SBPF_OK pc' rs' m') \<Longrightarrow> 
+  prog!(unat pc) = bins \<Longrightarrow>
+  \<forall> r \<noteq> dst. rs' r = rs r"
+  apply(cases bins,simp_all)
+  apply(cases "prog ! unat pc", simp_all)
+  subgoal for x91 apply(simp split:if_split_asm) 
+    apply(unfold eval_alu_def eval_reg_def,simp_all)
+    by auto
+  done
+
+lemma stack_is_not_changed_by_add:"Next spc' reg' m' = exec_instr xins sz spc reg m \<Longrightarrow> xins = Paddq_rr (bpf_to_x64_reg dst) (bpf_to_x64_reg src) 
+   \<Longrightarrow> match_stack reg m \<Longrightarrow> match_stack reg' m'"
+proof-
+  assume a0:"Next spc' reg' m' = exec_instr xins sz spc reg m" and
+  a1:"xins = Paddq_rr (bpf_to_x64_reg dst) (bpf_to_x64_reg src) " and
+  a2:"match_stack reg m"
+  have b0:"bpf_to_x64_reg dst \<noteq> RSP" using bpf_to_x64_reg_def by (cases dst,simp_all)
+  have b1:"reg SP = reg' SP" using exec_instr_def a0 a1 exec_instr_def b0 by simp
+  have b2:"m = m'" using a0 a1 exec_instr_def by force
+  have "match_stack reg' m'" using b1 b2 a2 match_stack_def by auto
+  thus ?thesis by blast
+qed
+
+lemma mem_is_not_changed_by_add:"Next spc' reg' m' = exec_instr xins sz spc reg m \<Longrightarrow> xins = Paddq_rr (bpf_to_x64_reg dst) (bpf_to_x64_reg src) 
+   \<Longrightarrow> m = m'"
+  using exec_instr_def by simp
+
+lemma addq_subgoal_rr_generic:
+  assumes a0:"bins = BPF_ALU64 BPF_ADD dst (SOReg src)" and
+       a1:"per_jit_add_reg64_1 dst src = Some (n, off, l_bin)" and
+       a3:"x64_decode 0 l_bin = Some (length l_bin, xins)" and
+       a4:"sbpf_step prog (SBPF_OK pc rs m) = (SBPF_OK pc' rs' m')" and
+       a5:"Next spc' reg' xm' = exec_instr xins sz spc reg xm" and
+       a6:"match_state (SBPF_OK pc rs m) (Next spc reg xm) " and
+       a7:"prog!(unat pc) = bins"
+  shows "match_state (SBPF_OK pc' rs' m') (Next spc' reg' xm') "
+proof -
+    have b0:"xins = Paddq_rr (bpf_to_x64_reg dst) (bpf_to_x64_reg src)" 
+      using x64_encode_decode_consistency per_jit_add_reg64_1_def a1 a3 list_in_list_prop
+    by (smt (verit, ccfv_SIG) Pair_inject map_option_eq_Some option.inject)
+    moreover have b1:"(\<forall> r. (rs r) = reg (bpf_to_x64_reg r))" using a6 spec match_state_def match_reg_def by simp
+    moreover have b2:"(rs src) = reg (bpf_to_x64_reg src)" using a6 spec b1 by simp
+    hence b3:"(rs' dst) = reg' (bpf_to_x64_reg dst)" using aluq_subgoal_rr_aux1 b0 b1 b2 a0 a4 a5 a7 by metis
+    have b4:"\<forall> r \<noteq> dst. reg'(bpf_to_x64_reg r) = reg (bpf_to_x64_reg r)" using b0 a5 aluq_subgoal_rr_aux2 by blast
+    have b5:"\<forall> r \<noteq> dst. (rs' r) = (rs r)" using aluq_subgoal_rr_aux3 a0 a4 a7 by force
+    have b6:"\<forall> r \<noteq> dst. (rs r) = reg ((bpf_to_x64_reg r))" using a6 using b1 by blast
+    have b7:"(\<forall> r \<noteq> dst. (rs' r) = reg' ((bpf_to_x64_reg r)))" using b1 b4 b5 by presburger
+    have b8:"match_stack reg' xm'" using stack_is_not_changed_by_add a6 match_state_def a5 b0 by simp
+    have b9:"match_mem m' xm'" using mem_is_not_changed mem_is_not_changed_by_add match_state_def a6
+      by (metis (no_types, lifting) a4 a5 b0 outcome.simps(4) sbpf_state.simps(9))
+    thus ?thesis using b3 b7 match_state_def b8 b9 match_reg_def by fastforce
+  qed
+      
+
+
+end
