theory/JITPer_aux.thy
@@ -1,0 +1,587 @@
+theory JITPer_aux
+imports
+  Main
+  rBPFCommType rBPFSyntax rBPFSem
+  x64Syntax x64Semantics x64Assembler Proof1
+  JIT_def
+begin
+
+record JitProgram =
+page_size     :: usize
+pc_section    :: "usize list"
+text_section  :: "x64_bin"
+
+record jit_state =
+jit_result :: JitProgram 
+offset_in_text_section :: usize 
+jit_pc :: usize
+
+abbreviation "REG_SCRATCH::ireg \<equiv> R11"
+
+definition bpf_to_x64_reg:: "bpf_ireg \<Rightarrow> ireg" where
+  "bpf_to_x64_reg br = (
+  case br of
+  BR0 \<Rightarrow> RAX |
+  BR1 \<Rightarrow> RDI |
+  BR2 \<Rightarrow> RSI |
+  BR3 \<Rightarrow> RDX |
+  BR4 \<Rightarrow> RCX |
+  BR5 \<Rightarrow> R8  |
+  BR6 \<Rightarrow> RBX |
+  BR7 \<Rightarrow> R13 |
+  BR8 \<Rightarrow> R14 |
+  BR9 \<Rightarrow> R15 |
+  BR10 \<Rightarrow> RBP
+)"
+
+lemma bpf_to_x64_reg_corr2[simp]:" bpf_to_x64_reg r1 \<noteq> bpf_to_x64_reg r2  \<longrightarrow> r1 \<noteq> r2 "
+  apply(unfold bpf_to_x64_reg_def)
+  apply(cases r1; cases r2; simp)
+  done
+
+lemma bpf_to_x64_reg_corr[simp]:" r1 \<noteq> r2 \<longrightarrow> bpf_to_x64_reg r1 \<noteq> bpf_to_x64_reg r2 "
+  apply(unfold bpf_to_x64_reg_def)
+  apply(cases r1; cases r2; simp)
+  done
+
+definition update_pc_section_aux ::"usize list \<Rightarrow> nat \<Rightarrow> usize \<Rightarrow> usize list" where
+"update_pc_section_aux pc_sec pc x = list_update pc_sec pc x"
+
+subsection \<open> JIT rule \<close>
+
+text \<open> return 
+  - the number of jited x64 assembly code
+  - the offset pointing to next pc
+  - the jited x64 binary code \<close>
+definition per_jit_add_reg64_1 :: "bpf_ireg \<Rightarrow> bpf_ireg \<Rightarrow> (nat \<times> u64 \<times> x64_bin) option" where
+"per_jit_add_reg64_1 dst src = (
+  let ins = Paddq_rr (bpf_to_x64_reg dst) (bpf_to_x64_reg src) in
+    Some (1, 1, x64_encode ins) 
+)"
+
+definition per_jit_exit :: "(nat \<times> u64 \<times> x64_bin) option" where
+"per_jit_exit = (
+  let ins = Pret in
+    Some (1, 1, x64_encode ins) 
+)"
+
+
+(*definition per_jit_mul_reg64::"bpf_ireg \<Rightarrow> bpf_ireg \<Rightarrow> (nat \<times> u64 \<times> x64_bin) option" where
+"per_jit_mul_reg64 dst src \<equiv> let ins_list = [Pmovq_rr (bpf_to_x64_reg src) R11, Ppushl_r RDX, Pmulq_r R11, Ppopl RDX] in
+   map_option (\<lambda> l. (5, 1, l)) (x64_encodes_func_suffix ins_list)"*)
+
+definition per_jit_mul_reg64::"bpf_ireg \<Rightarrow> bpf_ireg \<Rightarrow> (nat \<times> u64 \<times> x64_bin) option" where
+"per_jit_mul_reg64 dst src \<equiv> 
+  let ins_list = case (bpf_to_x64_reg dst) of 
+      RAX \<Rightarrow> (x64_encode (Pmovq_rr R11 (bpf_to_x64_reg src))@(x64_encode (Ppushl_r RDX)) @ (x64_encode (Pmulq_r R11)) @ (x64_encode (Ppopl RDX))) |
+      
+      RDX \<Rightarrow> (x64_encode (Pmovq_rr R11 (bpf_to_x64_reg src))@(x64_encode (Ppushl_r RAX)) @ (x64_encode (Pmovq_rr RAX RDX)) 
+                  @ (x64_encode (Pmulq_r R11))@ (x64_encode (Pmovq_rr RDX RAX))@ (x64_encode (Ppopl RAX)))|
+      
+      _   \<Rightarrow> (x64_encode(Pmovq_rr R11 (bpf_to_x64_reg src)))@(x64_encode (Ppushl_r RAX)) @ (x64_encode (Pmovq_rr RAX (bpf_to_x64_reg dst)))
+                  @ (x64_encode (Ppushl_r RDX)) @ (x64_encode (Pmulq_r R11)) @ (x64_encode (Ppopl RDX))
+                  @ (x64_encode (Pmovq_rr (bpf_to_x64_reg dst) RAX)) @ (x64_encode (Ppopl RAX))
+  in let len = case (bpf_to_x64_reg dst) of 
+    RAX \<Rightarrow> 4 |
+    RDX \<Rightarrow> 6 |
+    _ \<Rightarrow> 8
+    in Some (len, 1, ins_list)"
+
+                                               
+fun per_jit_ins ::" bpf_instruction \<Rightarrow> (nat \<times> u64 \<times> x64_bin) option" where
+"per_jit_ins bins = (
+  case bins of
+  BPF_ALU64 BPF_ADD dst (SOReg src) \<Rightarrow> (per_jit_add_reg64_1 dst src) |
+  BPF_EXIT \<Rightarrow> per_jit_exit |
+  BPF_ALU64 BPF_MUL dst (SOReg src) \<Rightarrow> (per_jit_mul_reg64 dst src) |
+  _ \<Rightarrow> None
+)"
+
+fun jitper :: "ebpf_asm \<Rightarrow> (nat \<times> u64 \<times> x64_bin) list option" where
+  "jitper [] = Some []" |
+  "jitper (h#xs) = (case per_jit_ins h of 
+                   None \<Rightarrow> None 
+                 | Some (n, off, x) \<Rightarrow> 
+                     (case jitper xs of 
+                        None \<Rightarrow> None 
+                      | Some res \<Rightarrow> Some ((n, off, x) # res)))"
+
+value "Some ((map the (map per_jit_ins [BPF_ALU64 BPF_ADD BR0 (SOReg BR6),BPF_ALU64 BPF_ADD BR0 (SOReg BR1)])))"
+
+value "jitper [BPF_ALU64 BPF_SUB BR0 (SOReg BR6),BPF_EXIT]"
+
+value "jitper [BPF_ALU64 BPF_MUL BR0 (SOReg BR6)]"
+
+                
+value "snd (snd ((the (jitper [BPF_EXIT,BPF_EXIT]))!(0::nat)))"
+
+value "jitper []"
+
+value "jitper [BPF_ALU64 BPF_SUB BR0 (SOReg BR6),BPF_ALU64 BPF_ADD BR0 (SOReg BR6)]"
+
+value "jitper [BPF_ALU64 BPF_ADD BR0 (SOReg BR6),BPF_ALU64 BPF_SUB BR0 (SOReg BR6)]"
+
+value "jitper [BPF_ALU64 BPF_ADD BR0 (SOReg BR6), BPF_ALU64 BPF_ADD BR0 (SOReg BR6), BPF_EXIT]"
+
+value "per_jit_ins (BPF_ALU64 BPF_ADD BR0 (SOReg BR6))"
+
+
+subsection \<open> simulation relation \<close>
+
+definition match_stack :: "regset \<Rightarrow> mem \<Rightarrow> bool" where
+"match_stack xrs m = (
+  \<exists> v. Mem.loadv M64 m (Vlong ((xrs SP) + (u64_of_memory_chunk M64))) = Some (Vlong v))" (* v of Vlong or Vint?*)
+
+text \<open> because jited x64 code may use pop and push to save registers,
+then x64 memory has more info than sbpf memory \<close>
+
+definition match_mem :: "mem \<Rightarrow> mem \<Rightarrow> bool" where
+"match_mem bm xm = (
+  \<forall> mc addr v. (Mem.loadv mc bm (Vlong addr) = Some v) \<longrightarrow> (Mem.loadv mc xm (Vlong addr) = Some v))"
+
+definition match_reg :: "reg_map \<Rightarrow> regset \<Rightarrow> bool" where
+  "match_reg rm rs = (\<forall> r. (rm r) = rs (bpf_to_x64_reg r))"
+
+definition match_state :: "sbpf_state \<Rightarrow> x64_state \<Rightarrow> bool" where
+"match_state bst xst = (
+  case bst of
+  SBPF_OK pc rs m \<Rightarrow> (
+    case xst of
+      Next xpc xrs xm \<Rightarrow>
+        match_reg rs xrs \<and> \<comment>\<open> for ALU + MEM + Call \<close>
+        match_mem m xm  \<comment>\<open> for MEM + Call \<close> \<and> 
+        match_stack xrs xm |
+      _ \<Rightarrow> False
+  ) |
+  SBPF_Success v \<Rightarrow>(
+    case xst of
+    Next xpc xrs xm \<Rightarrow> v = xrs (bpf_to_x64_reg BR0) \<comment>\<open> for EXIT \<close> |
+      _ \<Rightarrow> False
+  ) |
+  _ \<Rightarrow> False
+)"
+
+lemma sbpf_sem_induct: 
+  "sbpf_sem (m+n) prog s = s' \<Longrightarrow>
+    \<exists> temps.
+    sbpf_sem m prog s = temps \<and> 
+    sbpf_sem n prog temps = s'"
+  apply (induct m arbitrary: n prog s s')
+  apply simp_all
+  done
+
+lemma sbpf_sem_add: 
+  "sbpf_sem (m+n) prog s = s' \<Longrightarrow>
+    s = (SBPF_OK pc rs mem) \<Longrightarrow>
+    s'\<noteq> SBPF_Err \<Longrightarrow>
+    \<exists> temps.
+    sbpf_sem m prog s = temps \<and> 
+    sbpf_sem n prog temps = s'"
+  using sbpf_sem_induct by blast
+
+lemma sbpf_sem_err: 
+  "sbpf_sem (m+n) prog s = s' \<Longrightarrow>
+    s = SBPF_Err \<Longrightarrow>
+    \<exists> temps.
+    sbpf_sem m prog s = temps \<and> 
+    sbpf_sem n prog temps = s'"
+  using sbpf_sem_induct by blast
+
+lemma err_is_still_err:" sbpf_sem x prog SBPF_Err = s' \<Longrightarrow> s' = SBPF_Err "
+  apply(induct x, simp)
+  by auto
+
+lemma suc_success_is_err:"x > 0 \<Longrightarrow> sbpf_sem x prog (SBPF_Success v) = s' \<Longrightarrow> s' = SBPF_Err "
+  apply(induct x, simp)
+  using err_is_still_err by force
+
+lemma intermediate_step_is_ok:"sbpf_sem x prog s = s' \<Longrightarrow> x > 0 \<Longrightarrow> s' \<noteq> SBPF_Err \<Longrightarrow> \<exists> pc rs mem. s = (SBPF_OK pc rs mem)"
+  apply(induct x arbitrary: prog s s')
+  apply simp 
+  using err_is_still_err suc_success_is_err
+  by (metis sbpf_step.elims)
+
+
+
+lemma reg_r11_consist:"r = (bpf_to_x64_reg dst) \<Longrightarrow> r \<noteq> x64Syntax.R11"
+  apply(cases dst) 
+  by (unfold bpf_to_x64_reg_corr bpf_to_x64_reg_def, simp_all)
+
+lemma reg_rsp_consist:"r = (bpf_to_x64_reg dst) \<Longrightarrow> r \<noteq> x64Syntax.RSP"
+  apply(cases dst) 
+  by (unfold bpf_to_x64_reg_corr bpf_to_x64_reg_def, simp_all)
+
+lemma mem_is_not_changed:"s2 = sbpf_step prog s1 \<Longrightarrow> s1 = (SBPF_OK pc1 rs1 m1) \<Longrightarrow> s2 = (SBPF_OK pc2 rs2 m2) \<Longrightarrow> m1 = m2"
+  apply(cases "prog!(unat pc1)", simp_all)
+  subgoal for x11 x12 x13 
+    by (metis bpf_instruction.simps(361) sbpf_state.simps(6))
+  subgoal for x21 x22 x23 x24
+    by (metis bpf_instruction.simps(362) sbpf_state.simps(6))
+  subgoal for x31 x32 x33 x34 
+    by (metis bpf_instruction.simps(363) sbpf_state.simps(6))
+  subgoal for x4 
+    by (metis bpf_instruction.simps(364) sbpf_state.distinct(3))
+  subgoal for x51 x52 x53 
+    by (metis bpf_instruction.simps(365) sbpf_state.simps(6))
+  subgoal for x6 
+    by (metis bpf_instruction.simps(366) sbpf_state.simps(6))
+  subgoal for x71 x72
+    by (metis bpf_instruction.simps(367) sbpf_state.simps(6))
+  subgoal for x81 x82
+    by (metis bpf_instruction.simps(368) sbpf_state.simps(6))
+  subgoal for x91 x92 x93
+    apply(split if_splits, simp_all)
+    apply(split if_splits, simp_all)
+    apply(cases x91, simp_all)
+     apply(cases "eval_alu BPF_ADD x92 x93 rs1", simp_all)
+    apply(cases "eval_alu BPF_MUL x92 x93 rs1",simp_all)
+    done
+  subgoal for x10
+    by (metis bpf_instruction.simps(370) sbpf_state.simps(6))
+  subgoal for x111 x112
+    by (metis bpf_instruction.simps(371) sbpf_state.simps(6))
+  subgoal for x121 x122 x123
+    by (metis bpf_instruction.simps(372) sbpf_state.simps(6))
+  subgoal for x131 x132 x133
+    by (metis bpf_instruction.simps(373) sbpf_state.simps(6))
+  subgoal for x141 x142 x143
+    by (metis bpf_instruction.simps(374) sbpf_state.simps(6))
+  subgoal for x15
+    by (metis bpf_instruction.simps(375) sbpf_state.simps(6))
+  subgoal for x161 x162 x163 x164
+    by (metis bpf_instruction.simps(376) sbpf_state.simps(6))
+  subgoal for x171 x172
+    by (metis bpf_instruction.simps(377) sbpf_state.simps(6))
+  subgoal for x181 x182
+    by (metis bpf_instruction.simps(378) sbpf_state.simps(6))
+  by (metis (no_types, lifting) bpf_instruction.simps(379) sbpf_state.distinct(1) sbpf_state.simps(6))             
+
+(*lemma mem_is_not_changed2:"x64_sem 1 l xst1 = xst2 \<Longrightarrow> xst1 = Next xpc1 xrs1 m1 \<Longrightarrow> xst2 = Next xpc2 xrs2 m2 \<Longrightarrow> m1 = m2"
+  apply(cases "x64_decode (unat xpc1) l", simp_all)
+  subgoal for a apply(cases a, simp_all)
+    subgoal for aa b
+      apply(unfold exec_instr_def)
+      apply (cases b, simp_all)
+      apply(unfold exec_ret_def Let_def) 
+      apply(cases "loadv M64 m1 (xrs1 SP + u64_of_memory_chunk M64)", simp_all)
+      subgoal for ab apply(cases ab, simp_all)
+        done
+    done
+  done
+  done*)
+
+
+lemma aux1:"length prog \<noteq> 0 \<and> unat pc < length prog \<and> unat pc \<ge> 0 \<Longrightarrow> 
+  s' = sbpf_step prog s \<Longrightarrow>
+  s = (SBPF_OK pc rs m) \<Longrightarrow> 
+  s' = (SBPF_OK pc' rs' m') \<Longrightarrow> 
+  \<exists> dst src. prog!(unat pc) = BPF_ALU64 BPF_ADD dst (SOReg src) \<or> prog!(unat pc) = BPF_ALU64 BPF_MUL dst (SOReg src)"
+  apply(cases "prog!(unat pc)",simp_all)
+  subgoal for x91 x92 x93 
+   apply(unfold eval_alu_def Let_def)
+    apply(cases x91,simp_all) 
+     apply(cases x93, simp_all)
+     apply(cases x93, simp_all)
+    done
+  done
+
+lemma aux2:"length prog \<noteq> 0 \<and> unat pc < length prog \<and> unat pc \<ge> 0 \<Longrightarrow> 
+  s' = sbpf_step prog s \<Longrightarrow>
+  s = (SBPF_OK pc rs m) \<Longrightarrow> 
+  s' \<noteq> SBPF_Err \<Longrightarrow> 
+  \<exists> dst src. prog!(unat pc) \<in> {BPF_ALU64 BPF_ADD dst (SOReg src),BPF_EXIT, BPF_ALU64 BPF_MUL dst (SOReg src)}"
+  apply(cases "prog!(unat pc)",simp_all)
+  subgoal for x91 x92 x93 
+   apply(unfold eval_alu_def Let_def)
+    apply(cases x91,simp_all) 
+     apply(cases x93, simp_all)
+    apply(cases x93, simp_all)
+    done
+  done
+
+
+lemma aux3:"jitper prog = Some x64_prog \<Longrightarrow> length x64_prog = length prog"
+proof (induction prog arbitrary: x64_prog)
+  case Nil
+  then show ?case by simp
+next
+  case (Cons h xs)
+  assume "jitper (h # xs) = Some x64_prog"
+  then have a0:"\<exists> x. per_jit_ins h = Some x" using Cons(1) by (cases "per_jit_ins h"; auto)
+  obtain x where a1:"per_jit_ins h = Some x" using a0 by auto
+  then have a2:"\<exists> res. jitper xs = Some res" using Cons(1) apply (cases "jitper xs"; auto) 
+    using Cons.prems(1) by force
+  obtain res where a3:"jitper xs = Some res" using a2 by auto
+  have a4:" x64_prog = x # res" using Cons(1) a3 a1
+    using Cons.prems(1) by force
+  then have a5:"length ( x64_prog) = length (h # xs)" using a4 Cons.IH a3 by fastforce
+  then show ?case using Cons by simp
+qed
+
+
+value "[2::nat,3]!(unat (0::u64))"
+
+
+lemma aux5:"jitper prog = Some x64_prog \<Longrightarrow> unat pc \<ge> 0 \<and> unat pc < length prog \<Longrightarrow> 
+  prog!(unat pc) = bins \<Longrightarrow> x64_prog!(unat pc) = l_bin \<Longrightarrow> prog \<noteq> [] 
+  \<Longrightarrow> l_bin = the (per_jit_ins bins)"
+proof (induction prog arbitrary: x64_prog pc bins l_bin)
+  case Nil
+  then show ?case by simp
+next
+  case (Cons a prog)
+  then show ?case
+  proof-
+    have a0:"unat pc = 0 \<or> unat pc \<ge> 1" by auto
+    show ?thesis
+    proof (cases "unat pc = 0")
+      case True
+      have "unat pc = 0" using True a0 by simp
+      have b0:"\<exists> x. per_jit_ins a = Some x" using Cons by (cases "per_jit_ins a"; auto)
+      obtain x where b1:"per_jit_ins a = Some x" using b0 by auto
+      then have b2:"\<exists> res. jitper prog = Some res" using Cons(1) apply (cases "jitper prog"; auto) 
+        using Cons.prems(1) by force
+      obtain res where b3:"jitper prog = Some res" using b2 by auto
+      have b4:"x64_prog = x # res" using Cons(1) b3 b1 Cons by force
+      have bn:"l_bin = the (per_jit_ins bins)" using b1 b2 
+        using Cons.prems(3) Cons.prems(4) True b4 by fastforce
+      then show ?thesis using bn by blast
+    next
+      case False
+      have "\<exists> res. jitper prog = Some res" using Cons 
+        apply (cases "jitper prog"; simp_all) 
+        apply(cases a, simp_all) 
+        subgoal for x91 x92 x93 apply(cases x91,simp_all) 
+           apply(cases x93,simp_all)
+          subgoal for x2 apply(cases "per_jit_add_reg64_1 x92 x2",simp_all) 
+            done 
+          apply(cases x93,simp_all)
+          subgoal for x2 apply(cases "per_jit_mul_reg64 x92 x2",simp_all)
+            done 
+          done
+        apply(unfold per_jit_exit_def) 
+        apply(cases per_jit_exit,simp_all) 
+        done
+      then obtain res where b0:"jitper prog = Some res" by auto
+      have b1:"\<exists> x. per_jit_ins a = Some x" using Cons by (cases "per_jit_ins a"; auto)
+      obtain x where b2:"per_jit_ins a = Some x" using b1 by auto
+      have c0:" Some (x # res) = Some x64_prog" using b0 b2 Cons by auto
+      have c1:"unat pc \<ge> 1" using a0 False by blast
+      have c2:"(a#prog) ! unat pc = bins" using c0 Cons.prems(3) by blast
+      let "?pc'" = "unat pc -1"
+      have c4:"0 \<le> ?pc' \<and> ?pc' < length prog \<and>
+      prog ! ?pc' = bins \<and> res ! ?pc' = l_bin \<and> prog \<noteq> []" using Cons.prems(2) Cons.prems(3) Cons.prems(4) c0 c1 by auto
+      (* have cn:"0 \<le> unat pc \<and> unat pc < length prog \<Longrightarrow> 
+          prog ! unat pc = bins \<Longrightarrow> ?x ! unat pc = l_bin \<Longrightarrow> Some (snd (snd l_bin)) = per_jit_ins bins" using Cons
+        by (metis (no_types, lifting) jit.simps(2) option.case_eq_if option.collapse)*)
+      have c5:"l_bin = the (per_jit_ins bins)" using c4 Cons 
+         False jitper.simps(2) order_neq_le_trans unat_gt_0 unat_minus_one
+        by (metis (no_types, lifting) b0)
+      then show ?thesis using c5 by blast
+    qed
+  qed
+qed
+
+
+lemma corr_pc_aux1:"jitper prog = Some x64_prog \<Longrightarrow> 
+  prog \<noteq> [] \<and> unat pc \<ge> 0 \<and> unat pc < length prog \<Longrightarrow>
+  (num,off,l) = x64_prog!(unat pc) \<Longrightarrow>
+  off=1"
+proof (induction prog arbitrary: x64_prog pc num off l)
+  case Nil
+  then show ?case by simp
+next
+  case (Cons a prog)
+  then show ?case
+  proof-
+    have a0:"unat pc = 0 \<or> unat pc \<ge> 1" by auto
+    show ?thesis
+    proof (cases "unat pc = 0")
+      case True
+      have b0_1:"unat pc = 0" using True a0 by simp
+      have b0:"\<exists> x. per_jit_ins a = Some x" using Cons by (cases "per_jit_ins a"; auto)
+      obtain x where b1:"per_jit_ins a = Some x" using b0 by auto
+      have b1_1:"(num,off,l) = x" using b0_1 b1 True Cons
+        by (smt (verit) jitper.simps(2) nth_Cons_0 old.prod.case option.case_eq_if option.discI option.sel prod_cases3)
+      have bn:"off = 1" 
+        using b1 apply(cases "per_jit_ins a", simp_all) 
+        subgoal for aa 
+         apply(cases a,simp_all)
+        subgoal for x91 x92 x93
+          apply(cases x91,simp_all)
+          apply(cases x93,simp_all)
+          subgoal for x1 using b1 b1_1 per_jit_add_reg64_1_def Let_def by auto
+          apply(cases x93,simp_all) 
+          subgoal for x2 using b1 b1_1 per_jit_mul_reg64_def Let_def by auto
+          done
+        apply(unfold per_jit_exit_def Let_def, simp_all) using b1 b1_1 by blast
+      done
+      then show ?thesis using bn by blast
+    next
+      case False
+      have "\<exists> res. jitper prog = Some res" using Cons 
+        apply (cases "jitper prog"; simp_all) 
+        apply(cases a, simp_all) 
+        subgoal for x91 x92 x93 apply(cases x91,simp_all) 
+          apply(cases x93,simp_all)
+          subgoal for x2 apply(cases "per_jit_add_reg64_1 x92 x2",simp_all) 
+            done 
+          apply(cases x93,simp_all) 
+          subgoal for x2 apply(cases "per_jit_mul_reg64 x92 x2",simp_all) 
+            done
+          done
+        apply(unfold per_jit_exit_def) 
+        apply(cases per_jit_exit,simp_all) 
+        done
+      then obtain res where b0:"jitper prog = Some res" by auto
+      have b1:"\<exists> x. per_jit_ins a = Some x" using Cons by (cases "per_jit_ins a"; auto)
+      obtain x where b2:"per_jit_ins a = Some x" using b1 by auto
+      have c0:" Some (x # res) = Some x64_prog" using b0 b2 Cons by auto
+      have c1:"unat pc \<ge> 1" using a0 False by blast
+      have c2:"x64_prog ! unat pc = (num,off,l)" using c0 Cons by simp
+      let "?pc'" = "unat pc -1"
+      have c3:"(num,off,l) = res! ?pc'" using c0 False c2 by auto
+      have c4:"0 \<le> ?pc' \<and> ?pc' < length prog \<and> prog \<noteq> [] " using Cons c0 c1 by auto
+      have c5:"off=1" using c3 c4 
+        by (metis Cons.IH False b0 unat_minus_one unsigned_eq_0_iff)
+      then show ?thesis by blast
+    qed
+  qed
+qed
+
+
+lemma match_s_not_stuck:"match_state s xst \<Longrightarrow> xst \<noteq> Stuck"
+  apply(cases s, simp_all)
+  apply(unfold match_state_def)
+  subgoal for x11 x12 x13 by auto
+  subgoal for x2 by auto
+  by simp
+
+lemma x64_sem1_induct_aux1:"x64_sem1 (Suc n) pc x64_prog (Next xpc xrs m) = xst' \<Longrightarrow> 
+  x64_prog!(unat pc) = (num,off,l) \<Longrightarrow>
+  x64_sem num l (Next 0 xrs m) = xst1 \<Longrightarrow> 
+  x64_sem1 n (pc+off) x64_prog xst1 = xst'"
+ apply(induct n arbitrary:pc x64_prog xpc xrs m xst' num off l)
+ apply simp 
+  by simp
+
+lemma x64_sem1_induct_aux2:"x64_sem1 n pc x64_prog (Next xpc xrs xm) = x64_sem1 n pc x64_prog (Next 0 xrs xm)"
+proof(cases n)
+  case 0
+  then show ?thesis by simp
+next
+  case (Suc n)
+    thus ?thesis using Suc by fastforce
+qed
+ 
+lemma x64_sem1_induct_aux3:"
+  xst = (Next xpc xrs m) \<Longrightarrow>
+  x64_sem1 (Suc n) pc x64_prog xst = xst' \<Longrightarrow> 
+  x64_prog!(unat pc) = (num,off,l) \<Longrightarrow>
+  x64_sem num l (Next 0 xrs m) = xst1 \<Longrightarrow> 
+  xst1 = Next xpc1 xrs1 m1 \<Longrightarrow>
+  x64_sem1 n (pc+off) x64_prog (Next 0 xrs1 m1) = xst'"
+  using x64_sem1_induct_aux2 x64_sem1_induct_aux1 by metis
+
+lemma pc_scope_aux:"\<lbrakk> sbpf_sem n prog s = s'; s = (SBPF_OK pc rs m); s' = (SBPF_OK pc' rs' m'); prog \<noteq> []; n>0\<rbrakk> \<Longrightarrow> 
+  unat pc < length prog \<and> unat pc \<ge> 0"
+  by (metis (no_types, opaque_lifting) err_is_still_err linorder_not_less not_gr_zero sbpf_sem.elims sbpf_state.simps(6) sbpf_step.simps(1))
+
+(*
+lemma num_is_1_aux:"jitper prog = Some x64_prog \<Longrightarrow> prog \<noteq> [] \<and> unat pc < length prog \<and> 0 \<le> unat pc \<Longrightarrow> 
+  fst (x64_prog!(unat pc)) = 1"
+proof (induction prog arbitrary:x64_prog pc)
+  case Nil
+  then show ?case by blast
+next
+  case (Cons a prog)
+  then show ?case 
+  proof-
+    have a0:"unat pc = 0 \<or> unat pc \<ge> 1" by auto
+    have b0:"\<exists> x. per_jit_ins a = Some x" using Cons by (cases "per_jit_ins a"; auto)
+    obtain x where b1:"per_jit_ins a = Some x" using b0 by auto
+    then have b2:"\<exists> res. jitper prog = Some res" using Cons(1) apply (cases "jitper prog"; auto) 
+      using Cons.prems(1) by simp
+    obtain res where b3:"jitper prog = Some res"  using b2 by blast
+    have b4:"x64_prog = x # res" using Cons(1) b3 b1 Cons by force
+    show ?thesis
+    proof (cases "unat pc = 0")
+      case True
+      have b5:"unat pc = 0" using True a0 by simp
+      have b6:"fst (the (per_jit_ins a)) = 1"  
+        apply(cases "per_jit_ins a",simp_all)
+        using b1 apply fastforce
+        subgoal for aa apply(cases a,simp_all)
+          subgoal for x91 x92 x93
+            apply(cases x91, simp_all)
+            apply(cases x93,simp_all)
+            subgoal for x2 
+              apply(unfold per_jit_add_reg64_1_def Let_def,simp_all) 
+              using b5 by auto
+            done
+          apply(unfold per_jit_exit_def,simp_all)
+          using b5 by auto
+        done
+      have b7:"the (per_jit_ins a) = x64_prog!(unat pc)" using b5 b1 b4 by auto
+      then show ?thesis using b6 b7 by auto
+    next
+      case False
+      have c0:" Some (x # res) = Some x64_prog" using b4 by blast
+      have c1:"unat pc \<ge> 1" using a0 False by blast
+      let "?pc'" = "unat pc -1"
+      have c2:"0 \<le> ?pc' \<and> ?pc' < length prog \<and> prog \<noteq> []" using Cons 
+        by (metis False One_nat_def c1 length_Cons less_diff_conv2 less_one list.size(3) list.size(4) zero_le)
+      hence "fst (x64_prog ! unat pc) = 1" using c2 Cons False b3
+        by (metis (no_types, lifting) b4 nth_Cons' unat_minus_one unsigned_eq_0_iff)
+      then show ?thesis by blast
+    qed
+  qed
+qed
+*)
+
+
+lemma corr_pc_aux2:
+  "jitper prog = Some x64_prog \<Longrightarrow> prog \<noteq> [] \<and> unat pc \<ge> 0 \<and> unat pc < length prog \<Longrightarrow>
+  s =  SBPF_OK pc rs m \<Longrightarrow>
+  s' = sbpf_step prog s \<Longrightarrow> s' = SBPF_OK pc' rs' m' \<Longrightarrow> 
+  (num,off,l) = x64_prog!(unat pc) \<Longrightarrow>
+  pc' = pc+off"
+proof-
+  assume assm0:"s' = sbpf_step prog s"  and
+         assm1:"s' = SBPF_OK pc' rs' m'" and
+         assm2:"jitper prog = Some x64_prog" and
+         assm3:"prog \<noteq> [] \<and> unat pc \<ge> 0 \<and> unat pc < length prog" and
+         assm4:"s = SBPF_OK pc rs m" and
+         assm5:"(num,off,l) = x64_prog!(unat pc)"
+  have "\<exists> src dst. prog!(unat pc) \<in> {BPF_ALU64 BPF_ADD dst (SOReg src), BPF_ALU64 BPF_MUL dst (SOReg src), BPF_EXIT}" 
+    using assm0 assm1 assm3 assm4 aux2 length_0_conv sbpf_state.simps(6) by (smt (verit, del_insts) insert_commute)
+  then obtain src dst where c0:"prog!(unat pc) \<in> {BPF_ALU64 BPF_ADD dst (SOReg src), BPF_ALU64 BPF_MUL dst (SOReg src), BPF_EXIT}" by blast
+  have c1:"pc' = pc+1" using c0 assm0 assm1 apply(cases "prog!(unat pc)",simp_all)
+    prefer 2 using assm4 assm3 apply simp
+    subgoal for x91 x92 x93 apply(erule disjE)
+      using assm4 assm3 eval_alu_def apply simp 
+      using assm4 assm3 eval_alu_def by simp
+    done
+  have "off=1" 
+    using assm2 assm3 assm5 corr_pc_aux1 by blast
+  thus ?thesis using c1 by simp
+qed
+  (*have "x64_prog!(unat pc) = the (per_jit_ins (prog!(unat pc)))" using aux5 assm2 assm3 assm5 by blast
+  hence c2:"x64_prog!(unat pc) = the (per_jit_add_reg64_1 dst src) \<or> x64_prog!(unat pc) = the per_jit_exit" using c0 by auto
+  hence c3:"off = (fst(snd(the (per_jit_add_reg64_1 dst src)))) \<or> off = (fst(snd(the (per_jit_exit))))" using assm5 by (metis split_pairs)
+  thus ?thesis
+  proof(cases "off = (fst(snd(the (per_jit_exit))))")
+    case True
+    have "off = 1" using per_jit_add_reg64_1_def True by auto
+    then show ?thesis using c1 by simp
+  next
+    case True
+    have "off = (fst(snd(the (per_jit_exit))))" using True c3 by blast
+    hence "off = 1" using per_jit_exit_def Let_def try
+    then show ?thesis using c1 by simp
+  qed                                                   
+qed*)
+
+
+
+end
